Added a specific folder for DEX_I formalization

DEX_I/DEX_Framework.v
@@ -16,7 +16,7 @@ Variable observable : L.t.
 Variable PC : Set.
 Variable Method : Type.
 Variable Kind: Set.
-Variable step : Method -> PC -> (* Kind -> *) option PC -> Prop.
+Variable step : Method -> PC -> option PC -> Prop.
 Variable PM : Method -> Prop.
 Variable cdr : forall m, PM m -> CDR (step m).
 Implicit Arguments region.
@@ -29,28 +29,22 @@ Record SignedMethod : Type := SM {unSign:Method; sign:Sign}.
 Coercion unSign :  SignedMethod >-> Method.
 
 Variable istate rstate : Type.
-Variable exec : Method -> (* nat ->  Kind ->*) istate -> istate+rstate -> Prop.
+Variable exec : Method -> istate -> istate+rstate -> Prop.
 
 Variable pc : istate -> PC.
 
-Notation "m |- p1 => p2" := (step m p1 (* k *) (Some p2)) (at level 30). 
-Notation "m |- p1 => " := (step m p1 (* k *) None) (at level 30).
-Variable exec_step_some : forall m (* kd *) s s',
+Notation "m |- p1 => p2" := (step m p1 (Some p2)) (at level 30). 
+Notation "m |- p1 => " := (step m p1 None) (at level 30).
+Variable exec_step_some : forall m s s',
   PM m -> exec m (* kd *) s (inl _ s')-> m |- (pc s) => (pc s').
-Variable exec_step_none : forall m (* kd *) s s',
+Variable exec_step_none : forall m s s',
   PM m -> exec m (* kd *) s (inr _ s')-> m |- (pc s) =>.
 
 Variable registertypes : Type.
 
-(* Variable pbij : Set. *)
 Variable texec : forall m, PM m ->
-      Sign -> (PC->L.t) -> PC -> (* Kind ->   *)
+      Sign -> (PC->L.t) -> PC ->
       registertypes -> option registertypes -> Prop.
-(*
-Variable bexec :
-      Method -> Sign -> (PC->L.t) -> PC -> Kind ->  
-      istate -> stacktype -> pbij -> pbij -> Prop.
-*)
 Variable high_reg : registertypes -> Reg -> Prop.
 Variable indist_reg_val : istate -> istate -> Reg -> Prop.
 Variable indist_reg_val_trans : forall s1 s2 s3 r, 
@@ -64,10 +58,6 @@ Inductive indist_reg : registertypes -> registertypes -> istate -> istate -> Reg
 Variable indist : Sign -> registertypes -> registertypes -> istate -> istate -> Prop.
 Variable indist_from_reg : forall sgn rt1 rt2 s1 s2, 
   (forall r, indist_reg rt1 rt2 s1 s2 r) -> indist sgn rt1 rt2 s1 s2.
-(* Variable indist_reg_from_indist : forall sgn rt1 rt2 s1 s2,
-  indist sgn rt1 rt2 s1 s2 -> 
-    (forall r, high_reg rt1 r -> high_reg rt2 r -> indist_reg rt1 rt2 s1 s2 r) /\ 
-    (forall r, ~high_reg rt1 r \/ ~high_reg rt2 r -> indist_reg_val s1 s2 r). *)
 Variable indist_reg_from_indist : forall sgn rt1 rt2 s1 s2,
   indist sgn rt1 rt2 s1 s2 -> 
   forall r, 
@@ -76,58 +66,16 @@ Variable indist_reg_from_indist : forall sgn rt1 rt2 s1 s2,
       (high_reg rt1 r /\ ~high_reg rt2 r) \/
       (~high_reg rt1 r /\ high_reg rt2 r) ->
     indist_reg_val s1 s2 r).
-(* Variable irindist : Sign -> registertypes -> istate -> rstate -> Prop. *)
 Variable rindist : Sign -> rstate -> rstate -> Prop.
-(* Variable indist_trans :forall m rt1 rt2 rt3 s1 s2 s3,
- indist m rt1 rt2 s1 s2 -> 
- indist m rt2 rt3 s2 s3 -> 
- indist m rt1 rt3 s1 s3. *)
 Variable indist_sym : forall m rt1 rt2 s1 s2,
  indist m rt1 rt2 s1 s2 -> indist m rt2 rt1 s2 s1.
 Variable rindist_sym : forall m s1 s2,
  rindist m s1 s2 -> rindist m s2 s1.
 
-(* Variable indist_irindist_trans : forall m rt rt' s s' res res',
-  indist m rt rt' s s' ->
-  irindist m rt s res ->
-  irindist m rt' s' res' ->
-  rindist m res res'. *)
-
-(* Variable compat : Sign -> istate -> registertypes -> Prop.
-Variable compat_res : Sign -> rstate -> Prop. *)
-
 Variable high_result : Sign -> rstate -> Prop.
 
-(* Variable rt0 : Method -> Sign -> registertypes -> Prop. *)
 Variable rt0 : Method-> Sign -> registertypes.
-(* Variable init : Method -> istate -> Prop. *)
 Variable init_pc : Method -> PC -> Prop.
-(* Variable init_init_pc : forall m s, init m s -> init_pc m (pc s). *)
-
-
-(* Variable compat_init : forall m sgn s rt,
-  init m s -> rt0 m rt -> compat sgn s rt0. *)
-
-
-(* Variable high_opstack : stacktype -> istate -> Prop. *)
-
-(* Hendra 22082016 - focusin on DEX I
-Variable side_effect : Sign -> istate -> istate+rstate -> Prop.
-
-Variable side_effect_trans : forall m s1 s2 s3,
-  side_effect m s1 (inl _ s2) ->
-  side_effect m s2 s3 ->
-  side_effect m s1 s3.
-
-
-Inductive evalsto (m:Method) : nat -> nat -> istate -> rstate -> Prop :=
-  | evalsto_res : forall n k s res,
-      exec m n k s (inr _ res) -> evalsto m n 1 s res
-  | evalsto_intra : forall k n n1 n2 s1 s2 res,
-     exec m n1 k s1 (inl _ s2) -> 
-     evalsto m n2 n s2 res ->
-     evalsto m (S (n1+n2)) (S n) s1 res.
-*)
 
 Inductive evalsto (m:Method) : nat -> istate -> rstate -> Prop :=
   | evalsto_res : forall (* k *) s res,
@@ -141,32 +89,6 @@ Variable P : SignedMethod -> Prop.
 
 Variable PM_P : forall m, P m -> PM m.
 
-(* Definition cmp :=
-  forall m p sign s r rt,
-  P (SM m sign) ->
-  init_pc m (pc s) -> 
-  rt0 m sign rt ->
-  compat sign s rt ->
-  evalsto m p s r ->
-  compat_res sign r. *)
-
-
-(* Variable compat_exec_intra : forall sgn m se (* kd *) s s' rt rt', 
-(*   (forall k, k<n -> cmp k) -> *)
-  forall H0:P (SM m sgn),
-  exec m (* kd *) s (inl _ s') ->
-  texec m (PM_P _ H0) sgn se (pc s) (* kd *) rt (Some rt') ->
-  compat sgn s rt ->
-  compat sgn s' rt'. *)
-
-(* Variable compat_exec_return : forall sgn m se (* kd *) s r rt, 
-(*   (forall k, k<n -> cmp k) -> *)
-  forall H0:P (SM m sgn),
-  exec m (* kd *) s (inr _ r) ->
-  texec m (PM_P _ H0) sgn se (pc s) (* kd *) rt None ->
-  compat sgn s rt ->
-  compat_res sgn r. *)
-
 Definition ni :=
   forall m p p' sgn s s' r r',
   P (SM m sgn) ->
@@ -177,119 +99,69 @@ Definition ni :=
   init_pc m (pc s') ->
   evalsto m p s r ->
   evalsto m p' s' r' ->
-(*   compat sgn s rt ->
-  compat sgn s' rt -> *)
   rindist sgn r r'.
   
   
 (* seems weird to have same rt *)
-Variable indist2_intra : forall m sgn se rt ut ut' s s' u u' (* kd kd' *),
-(*   (forall k, k<N -> ni k) -> *)
-(*   ni ->  *)
+Variable indist2_intra : forall m sgn se rt ut ut' s s' u u',
   forall H0:P (SM m sgn), 
   indist sgn rt rt s s' ->
   pc s = pc s' ->
-  exec m (* kd *) s (inl _ u) ->
-  exec m (* kd' *) s' (inl _ u') ->
-  texec m (PM_P _ H0) sgn se (pc s) (* kd *) rt (Some ut) ->
-  texec m (PM_P _ H0) sgn se (pc s) (* kd' *) rt (Some ut') ->
-(*   compat sgn s rt ->
-  compat sgn s' rt -> *)
+  exec m s (inl _ u) ->
+  exec m s' (inl _ u') ->
+  texec m (PM_P _ H0) sgn se (pc s) rt (Some ut) ->
+  texec m (PM_P _ H0) sgn se (pc s) rt (Some ut') ->
     indist sgn ut ut' u u'.
 
-Variable indist2_return : forall m sgn se rt s s' u u' (* kd kd' *),
-(*   (forall k, k<N -> ni k) -> *)
+Variable indist2_return : forall m sgn se rt s s' u u',
   forall H0:P (SM m sgn),
   indist sgn rt rt s s' ->
   pc s = pc s' ->
-  exec m (* kd *) s (inr _ u) -> 
-  exec m (* kd' *) s' (inr _ u')-> 
-  texec m (PM_P _ H0) sgn se (pc s) (* kd *) rt None ->
-  texec m (PM_P _ H0) sgn se (pc s) (* kd' *) rt None ->
-(*   compat sgn s rt ->
-  compat sgn s' rt -> *)
+  exec m s (inr _ u) -> 
+  exec m s' (inr _ u')-> 
+  texec m (PM_P _ H0) sgn se (pc s) rt None ->
+  texec m (PM_P _ H0) sgn se (pc s) rt None ->
     rindist sgn u u'.
 
 (* high branching *)
-Variable soap2_basic_intra : forall m sgn se rt ut ut' s s' u u' (* kd kd' *),
-(*   (forall k, k<N -> ni k) -> *)
+Variable soap2_basic_intra : forall m sgn se rt ut ut' s s' u u',
   forall (h:P (SM m sgn)),
   indist sgn rt rt s s' -> 
   pc s = pc s' ->
-  exec m (* kd *) s (inl _ u) -> 
-  exec m (* kd' *) s' (inl _ u') -> 
-  texec m (PM_P _ h) sgn se (pc s) (* kd *) rt (Some ut) ->
-  texec m (PM_P _ h) sgn se (pc s) (* kd' *) rt (Some ut') ->
-(*   compat sgn s rt ->
-  compat sgn s' rt -> *)
+  exec m s (inl _ u) -> 
+  exec m s' (inl _ u') -> 
+  texec m (PM_P _ h) sgn se (pc s) rt (Some ut) ->
+  texec m (PM_P _ h) sgn se (pc s) rt (Some ut') ->
   pc u <> pc u' -> 
-(*   high_opstack ut u /\ *)
-  (forall j:PC, (region (cdr m (PM_P _ h)) (pc s) (* kd *) j) -> ~ leql (se j) observable).
-
-(* Variable soap2_basic_return : forall m sgn se rt ut s s' u u' (* kd kd' *),
-(*   (forall k, k<N -> ni k) -> *)
-  forall (h:P (SM m sgn)),
-  indist sgn rt rt s s' -> 
-  pc s = pc s' ->
-  exec m (* kd *) s (inl _ u) -> 
-  exec m (* kd' *) s' (inr _ u') -> 
-  texec m (PM_P _ h) sgn se (pc s) (* kd *) rt (Some ut) ->
-  texec m (PM_P _ h) sgn se (pc s) (* kd' *) rt None ->
-  compat sgn s rt ->
-  compat sgn s' rt ->
-(*   high_opstack ut u /\ *)
-  (forall j:PC, region (cdr m (PM_P _ h)) (pc s) (* kd *) j -> ~ leql (se j) observable)
-  (*    /\  
-  (forall j:PC, region (cdr m (PM_P _ h)) (pc s) (* kd' *) j -> ~ leql (se j) observable) *). *)
+    (forall j:PC, (region (cdr m (PM_P _ h)) (pc s) j) -> ~ leql (se j) observable).
 
 Variable sub : registertypes -> registertypes -> Prop.
-(* Variable sub_high_opstack : forall st1 st2 s,
-  high_opstack st1 s -> sub st1 st2 -> high_opstack st2 s. *)
-(* Variable sub_double : forall sgn st1 st2 st s1 s2 b1 b2,
-  indist sgn st1 st2 b1 b2 s1 s2 ->
-  sub st1 st -> sub st2 st ->
-  indist sgn st st b1 b2 s1 s2. *)
 Variable sub_simple : forall sgn rt rt' rt0 s s0,
   indist sgn rt0 rt s0 s ->
-  sub rt rt' -> (* high_opstack st s -> *)
+  sub rt rt' ->
   indist sgn rt0 rt' s0 s.
-(* Variable indist_high_opstack : forall sgn st1 st2 st1' st2' b1 b2 s1 s2,
-  indist sgn st1 st2 b1 b2 s1 s2 ->
-  high_opstack st1' s1 ->
-  high_opstack st2' s2 ->
-  indist sgn st1' st2' b1 b2 s1 s2. *)
-(* Variable sub_irindist : forall sgn rt rt' s1 s2,
-  irindist sgn rt s1 s2 -> sub rt rt' ->
-  irindist sgn rt' s1 s2. *)
-(* Variable sub_compat : forall sgn s rt1 rt2,
-  sub rt1 rt2 ->
-  compat sgn s rt1 ->
-  compat sgn s rt2. *)
 
 Inductive typed_exec (m:Method) (H:PM m) (sgn:Sign) (se:PC->L.t) (RT:PC->registertypes) 
-: (* nat ->  Kind ->*) istate -> istate + rstate -> Prop :=
-  typed_exec_def1 : forall (* kd *) s1 s2 rt',
-   exec m (* kd *) s1 (inl _ s2) ->
+: istate -> istate + rstate -> Prop :=
+  typed_exec_def1 : forall s1 s2 rt',
+   exec m s1 (inl _ s2) ->
    sub rt' (RT (pc s2)) ->
-   texec m H sgn se (pc s1) (* kd *) (RT (pc s1)) (Some rt') ->
-   typed_exec m H sgn se RT (* kd *) s1 (inl _ s2)
-| big_exec_def2 : forall (* kd *) s1 s2,
-   exec m (* kd *) s1 (inr _ s2) ->
-   texec m H sgn se (pc s1) (* kd *) (RT (pc s1)) None ->
-   typed_exec m H sgn se RT (* kd *) s1 (inr _ s2).
+   texec m H sgn se (pc s1) (RT (pc s1)) (Some rt') ->
+   typed_exec m H sgn se RT s1 (inl _ s2)
+| big_exec_def2 : forall s1 s2,
+   exec m s1 (inr _ s2) ->
+   texec m H sgn se (pc s1) (RT (pc s1)) None ->
+   typed_exec m H sgn se RT s1 (inr _ s2).
 
-Inductive tevalsto (m:Method) (H:PM m) (sgn:Sign) (se:PC->L.t) (RT:PC->registertypes) : nat -> (* nat -> *) istate -> rstate -> Prop :=
-  | tevalsto_res : forall (* k *) s res,
-      typed_exec m H sgn se RT (* k *) s (inr _ res) -> tevalsto m H sgn se RT 1 s res
-  | tevalsto_intra : forall (* k *) n s1 s2 res,
-     typed_exec m H sgn se RT (* k *) s1 (inl _ s2) -> 
+Inductive tevalsto (m:Method) (H:PM m) (sgn:Sign) (se:PC->L.t) (RT:PC->registertypes) : nat -> istate -> rstate -> Prop :=
+  | tevalsto_res : forall s res,
+      typed_exec m H sgn se RT s (inr _ res) -> tevalsto m H sgn se RT 1 s res
+  | tevalsto_intra : forall n s1 s2 res,
+     typed_exec m H sgn se RT s1 (inl _ s2) -> 
      tevalsto m H sgn se RT n s2 res ->
      tevalsto m H sgn se RT (S n) s1 res.
 
 (* Hendra additional *)
-(* Variable tevalsto_high_result : forall m sgn (H:PM m) se RT s res,
-  ~L.leql (se (pc s)) observable ->
-  tevalsto m H sgn se RT 1 s res -> high_result sgn res. *)
 Variable tevalsto_high_result' : forall m sgn (H:PM m) se s RT res,
   ~L.leql (se m sgn (pc s)) observable ->
   exec m s (inr res) ->
@@ -300,18 +172,8 @@ Variable tevalsto_diff_high_result : forall se RT m sgn s s' p res res' (H:PM m)
   tevalsto m H sgn (se m sgn) (RT m sgn) 1 s res -> tevalsto m H sgn (se m sgn) (RT m sgn) p s' res' -> 
   high_result sgn res /\ high_result sgn res'.
 
-(* Variable tevalsto_high_result2 : forall m (H:PM m) sgn se RT s u res,
-  high_region m H sgn (pc s) ->
-  region (cdr m (PM_P _ H)) (pc s)  *)
-
 Variable high_result_indist : forall sgn res res0,
   high_result sgn res -> high_result sgn res0 -> rindist sgn res res0.
-
-(* Variable high_result_implies_high_result : forall m sgn p p' s s' res res' (H: P (SM m sgn)),
-  evalsto m p s res ->
-  evalsto m p' s' res' ->
-  high_result sgn res -> high_result sgn res'. *)
-(* *)
 
 Variable eq_map : registertypes -> registertypes -> Prop.
 Variable eq_map_refl : reflexive registertypes eq_map.
@@ -331,20 +193,15 @@ forall x0 y1 : registertypes,
 eq_map x0 y1 -> forall y2 y3 : istate, indist y x x0 y2 y3 <-> indist y y0 y1 y2 y3.
 Add Morphism indist : indist_morphism. Proof. exact indist_morphism_proof. Qed.
 
-(* Variable compat_morphism_proof : forall (y : Sign) (y0 : istate) (x y1 : registertypes),
-eq_map x y1 -> compat y y0 x <-> compat y y0 y1.
-Add Morphism compat : compat_morphism. Proof. exact compat_morphism_proof. Qed. *)
-
 Definition Typable (m:Method) (H:PM m) (sgn:Sign) (se:Method->Sign->PC->L.t) (RT:Method->Sign->PC->registertypes) : Prop :=
   (forall i, init_pc m i -> eq_map (RT m sgn i) (rt0 m sgn)) /\ 
-(*   (forall s1 s2, init_pc m (pc s1) -> init_pc m (pc s2) -> indist sgn (RT m sgn (pc s1)) (RT m sgn (pc s2)) s1 s2) /\ *)
-  (forall i (* kd *),
-     m |- i =>(*kd*) ->
-     texec m H sgn (se m sgn) i (* kd *) (RT m sgn i) None) /\
-  (forall i j (* kd *),
-    m |- i =>(*kd*) j ->
+  (forall i,
+     m |- i => ->
+     texec m H sgn (se m sgn) i (RT m sgn i) None) /\
+  (forall i j,
+    m |- i =>j ->
     exists rt,
-      texec m H sgn (se m sgn) i (* kd *) (RT m sgn i) (Some rt) 
+      texec m H sgn (se m sgn) i (RT m sgn i) (Some rt) 
       /\ sub rt (RT m sgn j)).
 
 Definition TypableProg se S := 
@@ -360,13 +217,13 @@ Proof.
   destruct H as [_ [H0 H1]].
   induction 1.
   (* ret *)
-  constructor 1 (* with k *); auto.
+  constructor 1; auto.
   constructor; auto.
   apply H0; auto.
   eapply exec_step_none; eauto.
   (* next *)
-  constructor 2 with (* k *) s2; auto.  
-  elim H1 with (pc s1) (pc s2) (* k *).
+  constructor 2 with s2; auto.  
+  elim H1 with (pc s1) (pc s2).
   intros st (HT,Hs).
   constructor 1 with st; auto.
   eapply exec_step_some; eauto.  
@@ -379,11 +236,9 @@ Lemma tevalsto_evalsto : forall se RT m sgn p s r
 Proof.
   induction 1.
   inversion H. 
-(*    inversion_mine H;  *)
-  constructor 1 (* with k *); auto.
-(*   inversion_mine H. *)
+  constructor 1; auto.
   inversion H.
-  constructor 2 with (* k *) s2; auto. 
+  constructor 2 with s2; auto. 
 Qed.
 
 Lemma tevalsto_high_result : forall m sgn (H:PM m) se RT s res,
@@ -398,147 +253,57 @@ Qed.
 
 Implicit Arguments tevalsto_evalsto.
 
-(* Definition wf_eval se RT :=
-  forall m sgn s r p (H:P (SM m sgn)),
-  tevalsto m (PM_P _ H) sgn (se m sgn) (RT m sgn) p s r ->
-  compat sgn s (RT m sgn (pc s)) ->
-  compat_res sgn r. *)
-
 Hint Resolve PM_P.
-
-(* Lemma wf_eval_cmp : forall se RT,
-  TypableProg se RT ->
-  wf_eval se RT ->
-  cmp.
-Proof.
-  unfold wf_eval, cmp; intros.
-  apply H0 with m s p H1; auto.
-  apply typable_evalsto; auto.
-  destruct (H _ _ H1) as [T1 _].
-  rewrite T1 with (rt:=rt); auto.
-Qed. *)
- 
-(* Lemma wf_eval_induction : forall se RT,
-  TypableProg se RT -> 
-  wf_eval se RT.
-Proof.
-  intros se RT H.
- (*  apply lt_wf_ind; auto.
-  apply lt_wf_ind; clear n; intros. *)
-  unfold wf_eval.
-  induction 1; intros. 
-  inversion H1. subst.
-  apply compat_exec_return with (2:=H6) (3:=H2); auto.
-  inversion H1; subst.
-  apply IHtevalsto.
-  apply sub_compat with (rt1:=rt'); auto.
-  apply compat_exec_intra with m (se m sgn) (* k  *)s1 (RT m sgn (pc s1)) H0; auto.
-Qed.  *)
-
-(* Lemma safe_cmp : forall se RT rt,
-  TypableProg se RT -> 
-  forall m sign s r p (h:P (SM m sign)),
-  init_pc m (pc s) -> 
-  rt0 m sign rt ->
-  compat sign s rt ->
-  evalsto m p s r ->
-  compat_res sign r.
-Proof.
-  intros.
-  generalize (wf_eval_cmp se RT); unfold cmp; intros.
-  eapply H4; eauto.
-  apply wf_eval_induction; auto.
-Qed. *)
 
 Section TypableProg.
 Variable se : Method -> Sign -> PC -> L.t.
 Variable RT : Method -> Sign -> PC -> registertypes.
 Variable T : TypableProg se RT.
 
-Definition high_region m (h:PM m) sgn (i:PC) (*kd:Kind*) := 
-  forall j:PC, region (cdr m h) i (* kd *) j ->
+Definition high_region m (h:PM m) sgn (i:PC) := 
+  forall j:PC, region (cdr m h) i j ->
     ~ leql (se m sgn j) observable.
 
-(* Lemma wf_prop : forall m sgn s r p,
-  P (SM m sgn) ->
-  evalsto m p s r -> 
-  compat sgn s (RT m sgn (pc s))->
-  compat_res sgn r.
-Proof.
-  intros.
-  apply (wf_eval_induction _ _ T m sgn s r p H); auto.
-  apply typable_evalsto; auto.
-Qed. *)
-
-(* Lemma wf_step_intra : forall m sgn (* k *) s1 s2,
-  P (SM m sgn) ->
-  compat sgn s1 (RT m sgn (pc s1)) ->
-  exec m (* k *) s1 (inl _ s2) -> 
-  compat sgn s2 (RT m sgn (pc s2)).
-Proof.
-  intros.
-  destruct (T _ _ H) as [U1 [U2 U3]].
-  destruct (U3 (pc s1) (pc s2) (* k *)) as [rt [P1 P2]].
-  eapply exec_step_some; eauto.
-  apply PM_P with (1:=H).
-  apply sub_compat with rt; auto.
-  apply compat_exec_intra with m (se m sgn) (* k *) s1 (RT m sgn (pc s1)) H; auto.
-  (* intros; apply wf_eval_cmp with se S; auto.
-  apply wf_eval_induction; auto. *)
-Qed. *)
-
 Hint Immediate indist_sym rindist_sym.
-Hint Resolve exec_step_some (* wf_step_intra *) exec_step_none.
+Hint Resolve exec_step_some exec_step_none.
 
-Lemma final_bighighstep_aux : forall m sgn i p s res (* kd *) (H: P (SM m sgn)),
-(*   compat sgn s (RT m sgn (pc s)) -> *)
+Lemma final_bighighstep_aux : forall m sgn i p s res (H: P (SM m sgn)),
   tevalsto m (PM_P _ H) sgn (se m sgn) (RT m sgn) p s res ->
-  region (cdr m (PM_P _ H)) i (* kd *) (pc s) ->
-  (forall jun, ~junc (cdr m (PM_P _ H)) i (* kd *) jun) ->
-  high_region m (PM_P _ H) sgn i (* kd *) ->
+  region (cdr m (PM_P _ H)) i (pc s) ->
+  (forall jun, ~junc (cdr m (PM_P _ H)) i jun) ->
+  high_region m (PM_P _ H) sgn i ->
   high_result sgn res.
 Proof.
   intros.
   induction H0.
   apply tevalsto_high_result with (m:=m) (H:=(PM_P _ H)) (se:=se) (RT:=RT) (s:=s); auto.
-    constructor 1 (* with (k:=k) *); auto.
+    constructor 1; auto.
   apply IHtevalsto; auto.
   inversion H0.
-(*     apply sub_compat with (s:=s2) (rt1:=rt') (rt2:=RT m sgn (pc s2)); auto. *)
-(*     apply compat_exec_intra with (m:=m) (se:=se m sgn) (*kd:=k*) (s:=s1) (s':=s2)  *)
-(*       (rt:=RT m sgn (pc s1)) (rt':=rt') (H0:=H); auto. *)
-(*   inversion H1.  *)
     eapply exec_step_some with (1:=PM_P _ H) in H6; eauto.
-    elim (soap2 (cdr m (PM_P _ H))) with i (pc s1) (pc s2) (* k  kd*); auto.
+    elim (soap2 (cdr m (PM_P _ H))) with i (pc s1) (pc s2); auto.
     intros. unfold not in H2. apply H2 in H10. contradiction.
 Qed.
 
-Lemma final_bighighstep : forall m sgn p i s0 s res res0 (*kd kd'*)
+Lemma final_bighighstep : forall m sgn p i s0 s res res0
   (H:P (SM m sgn)),
   pc s = pc s0 ->
-  (* compat sgn s (RT m sgn (pc s)) -> 
-  compat sgn s0 (RT m sgn (pc s)) -> *)
   evalsto m p s res-> 
   evalsto m 1 s0 res0 ->
-  region (cdr m (PM_P _ H)) i (* kd  *) (pc s)-> 
+  region (cdr m (PM_P _ H)) i (pc s)-> 
   indist sgn (RT m sgn (pc s)) (RT m sgn (pc s0)) s s0 ->
-  high_region m (PM_P _ H) sgn i (* kd *) ->
-(*   high_opstack (S m sgn (pc s)) s -> *)
-(*   step m i kd' None ->  *)
-  rindist sgn res res0.
+  high_region m (PM_P _ H) sgn i ->
+    rindist sgn res res0.
 Proof.
   intros.
-  (* apply typable_evalsto with (1:=T m sgn H) in H3.
-  apply typable_evalsto with (1:=T m sgn H) in H4. *)
   inversion H2; try (inversion H8).
   destruct (T m sgn H). inversion_mine H11.
   apply high_result_indist.
   (* high result res *)
-    apply final_bighighstep_aux with (m:=m) (i:=i) (p:=p) (s:=s) (*kd:=kd*) (H:=H); auto.
+    apply final_bighighstep_aux with (m:=m) (i:=i) (p:=p) (s:=s) (H:=H); auto.
     apply typable_evalsto; auto.
     intros.
     apply soap3 with (j:=pc s0).
-(*     elim (soap3 (cdr m (PM_P _ H))) with i (pc s0) jun kd; auto.  *)
     rewrite <- H0; auto.
     apply exec_step_none with (1:=PM_P _ H) in H6.
     unfold result; eauto.
@@ -655,9 +420,6 @@ Proof.
   rewrite H0 in H6; auto.
 Qed.
 
-(* Inductive path (m:Method) (i:PC) : PC -> Prop :=
-  | path_base : forall j, j = i -> path m i j 
-  | path_step : forall j k, path m k j -> step m i (Some k) -> path m i j. *)
 Inductive path (m:Method) (i:istate) : istate -> Type :=
   | path_base : forall j, exec m i (inl j) -> path m i j 
   | path_step : forall j k, path m k j -> exec m i (inl k) -> path m i j.
@@ -670,25 +432,17 @@ Inductive path_in_region (m:Method) (cdr: CDR (step m)) (s:PC) (i j:istate) : (p
   | path_in_reg_ind : forall k (Hexec:exec m i (inl k)) (p:path m k j), region cdr s (pc i) ->
       path_in_region m cdr s k j p -> path_in_region m cdr s i j (path_step m i j k p Hexec).
 
-(* Inductive path (m:Method) (sgn:Sign) (H:PM m) (i:istate) : istate -> Prop :=
-  | path_base : forall j ort, texec m H sgn (se m sgn) (pc i) (RT m sgn (pc i)) ort -> 
-      exec m i (inl j) -> path m sgn H i j 
-  | path_step : forall j k ort, path m sgn H k j -> exec m i (inl k) -> 
-      texec m H sgn (se m sgn) (pc i) (RT m sgn (pc i)) ort -> path m sgn H i j.
- *)
 Lemma evalsto_path : forall m sgn n s i res (H: P (SM m sgn)),
   region (cdr m (PM_P _ H)) s (pc i) ->
-(*   compat sgn i (RT m sgn (pc i)) -> *)
   evalsto m n i res ->
   (exists j p, junc (cdr m (PM_P _ H)) s (pc j) /\ path_prop m i j p /\
     path_in_region m (cdr m (PM_P _ H)) s i j p /\
-(*     compat sgn j (RT m sgn (pc j)) /\  *)
     (exists n', evalsto m n' j res /\ n' < n)) 
   \/ (forall jun, ~junc (cdr m (PM_P _ H)) s jun).
 Proof.
   intros m sgn n. pattern n. apply lt_wf_ind.
   clear n. intros n IH.
-  intros s i res H Hreg (* Hcompat *) Hevalsto.
+  intros s i res H Hreg Hevalsto.
   inversion Hevalsto.
   (* the case where i is immediately a return point *)
   apply exec_step_none with (1:=PM_P _ H) in H0.
@@ -704,81 +458,34 @@ Proof.
   constructor 2; auto.
   exists x1. split; auto.
   omega.
- (*  destruct (T m sgn H). Cleanexand.
-  assert (H0':=H0).
-  apply exec_step_some with (1:=PM_P _ H) in H0. 
-  specialize H4 with (i:=pc i) (j:=pc s2) (1:=H0).
-  Cleanexand.
-  constructor 2 with (k:=s2) (ort:=Some x1); auto.
-(*   auto.
-  apply exec_step_some with (1:=PM_P _ H); auto. *)
-  exists x0. split; auto.
-  omega. *)
-  (* (* compat *)
-  destruct (T m sgn H).
-  Cleanexand.
-  assert (H0':=H0).
-  apply exec_step_some with (1:=PM_P _ H) in H0.
-  specialize H8 with (i:=pc i) (j:=pc s2) (1:=H0).
-  destruct H8.
-  Cleanexand.
-  apply sub_compat with (rt1:=x); auto.
-  apply compat_exec_intra with (m:=m) (se:=se m sgn) (s:=i) (rt:=RT m sgn (pc i)) (H0:=H); auto. *)
+
   (* path is the junction *) 
   left. exists s2. exists (path_base m i s2 H0).
   repeat (split; auto).
   constructor 1; auto. 
-  (* (* *)
-  assert (H0':=H0).
-  apply exec_step_some with (1:=PM_P _ H) in H0. 
-  destruct (T m sgn H). Cleanexand.
-  specialize H8 with (i:=pc i) (j:=pc s2) (1:=H0). Cleanexand.
-  constructor 1 with (j:=s2) (ort:=Some x); auto. (* apply exec_step_some with (1:=PM_P _ H) in H0; auto. *)
-  (* (* *)
-  constructor 2 with (k:=pc s2); auto. constructor; auto.
-  apply exec_step_some with (1:=PM_P _ H); auto. *) *)
-  (* (* compat *)
-  destruct (T m sgn H).
-  Cleanexand.
-  assert (H0':=H0).
-  apply exec_step_some with (1:=PM_P _ H) in H0.
-  specialize H8 with (i:=pc i) (j:=pc s2) (1:=H0).
-  destruct H8.
-  Cleanexand.
-  apply sub_compat with (rt1:=x); auto.
-  apply compat_exec_intra with (m:=m) (se:=se m sgn) (s:=i) (rt:=RT m sgn (pc i)) (H0:=H); auto. *)
+
   (* final case *)
   exists n0; repeat (split; auto).
   apply exec_step_some with (1:=PM_P _ H); auto.
 Qed.
 
 Variable changed : forall (m:Method) (i j:istate), path m i j -> Reg -> Prop.
-(* Variable changed_high : forall m sgn s i j r (H: P (SM m sgn)), 
-  (forall k:PC, region (cdr m (PM_P _ H)) s (* kd *) k -> ~ L.leql (se m sgn k) observable) ->
-  region (cdr m (PM_P _ H)) s i ->
-  junc (cdr m (PM_P _ H)) s (pc j) ->
-  path m i j -> 
-  changed i j r -> high_reg (RT m sgn j) r. *)
-Variable changed_high : forall m sgn s i j r (H:P (SM m sgn)) (Hpath: path m (* sgn (PM_P _ H) *) i j), 
-  (forall k:PC, region (cdr m (PM_P _ H)) s (* kd *) k -> ~ L.leql (se m sgn k) observable) ->
+Variable changed_high : forall m sgn s i j r (H:P (SM m sgn)) (Hpath: path m i j), 
+  (forall k:PC, region (cdr m (PM_P _ H)) s k -> ~ L.leql (se m sgn k) observable) ->
   path_in_region m (cdr m (PM_P _ H)) s i j Hpath ->
   region (cdr m (PM_P _ H)) s (pc i) ->
   junc (cdr m (PM_P _ H)) s (pc j) ->
-(*   In r (VarMap.dom _ (RT m sgn (pc j))) -> *)
-  changed m (* sgn (PM_P _ H) *) i j Hpath r -> high_reg (RT m sgn (pc j)) r.
-(* Variable not_changed_same : forall m sgn i j r s1 s2 (H: P (SM m sgn)),
-  path m i j -> ~changed i j r -> 
-  pc (s1) = i -> pc (s2) = j ->
-  (~high_reg (RT m sgn i) r -> indist_reg_val s1 s2 r) /\ (high_reg (RT m sgn i) r -> high_reg (RT m sgn j) r).  *)
+  changed m i j Hpath r -> 
+    high_reg (RT m sgn (pc j)) r.
 Variable not_changed_same : forall m sgn i j (Hpath: path m i j) r (H: P (SM m sgn)) ,
   ~changed m i j Hpath r -> 
-  (indist_reg_val i j r) /\ (high_reg (RT m sgn (pc i)) r -> high_reg (RT m sgn (pc j)) r). 
+  (indist_reg_val i j r) /\ (high_reg (RT m sgn (pc i)) r -> 
+    high_reg (RT m sgn (pc j)) r). 
 Variable high_reg_dec : forall rt r, high_reg rt r \/ ~high_reg rt r.
 Variable changed_dec : forall m i j r (p:path m i j),
   changed m i j (p) r \/ ~changed m i j (p) r. 
 
 Lemma junction_indist : forall m sgn ns ns' s s' u u' res res' i (H: P (SM m sgn)),
-(*   compat sgn s (RT m sgn (pc s)) -> compat sgn s' (RT m sgn (pc s')) ->   *)
   indist sgn (RT m sgn (pc s)) (RT m sgn (pc s')) s s' ->
   exec m s (inl u) -> exec m s' (inl u') ->
   region (cdr m (PM_P _ H)) i (pc u) ->
@@ -792,34 +499,12 @@ Lemma junction_indist : forall m sgn ns ns' s s' u u' res res' i (H: P (SM m sgn
     evalsto m ps' v' res' /\ ps' <= ns' /\
     junc (cdr m (PM_P _ H)) i (pc v) /\ 
     junc (cdr m (PM_P _ H)) i (pc v') /\
-(*     compat sgn v (RT m sgn (pc v)) /\ compat sgn v' (RT m sgn (pc v')) /\  *)
     indist sgn (RT m sgn (pc v)) (RT m sgn (pc v')) v v')
   \/ (high_result sgn res /\ high_result sgn res'). 
 Proof.
   intros.
-  (* assert (compat sgn u (RT m sgn (pc u))).
-    destruct (T m sgn H).
-    Cleanexand.
-    assert (H3':=H3).
-    apply exec_step_some with (1:=PM_P _ H) in H3.
-    specialize H13 with (i:=pc s) (j:=pc u) (1:=H3).
-    destruct H13.
-    Cleanexand.
-    apply sub_compat with (rt1:=x); auto.
-    apply compat_exec_intra with (m:=m) (se:=se m sgn) (s:=s) (rt:=RT m sgn (pc s)) (H0:=H); auto.
-  assert (compat sgn u' (RT m sgn (pc u'))).
-    destruct (T m sgn H).
-    Cleanexand.
-    assert (H4':=H4).
-    apply exec_step_some with (1:=PM_P _ H) in H4.
-    specialize H14 with (i:=pc s') (j:=pc u') (1:=H4).
-    destruct H14.
-    Cleanexand.
-    apply sub_compat with (rt1:=x); auto.
-    apply compat_exec_intra with (m:=m) (se:=se m sgn) (s:=s') (rt:=RT m sgn (pc s')) (H0:=H); auto.
- *)
-  elim evalsto_path with (1:=H3) (* (2:=H11)  *) (2:=H6); 
-  elim evalsto_path with (1:=H4) (* (2:=H12)  *) (2:=H7); intros.
+  elim evalsto_path with (1:=H3) (2:=H6); 
+  elim evalsto_path with (1:=H4) (2:=H7); intros.
   left. destruct H10 as [v H10]; destruct H10 as [path H10]; destruct H9 as [v' H9]; destruct H9 as [path' H9].
     exists v; exists v'.
     Cleanexand.
@@ -858,7 +543,6 @@ Proof.
     elim junc_func with (PC:=PC) (step:=step m) (c:=cdr m (PM_P _ H)) (i:=i) 
       (j1:=pc v') (j2:=pc v); auto.
     constructor 1; auto.
-(*     specialize H25 with (1:=H30); specialize H27 with (1:=H29). *)
     constructor 2; auto.
     apply indist_reg_val_trans with (s2:=u).
     apply indist_reg_val_sym; auto.
@@ -882,7 +566,6 @@ Proof.
 Qed.
 
 Lemma junction_indist_2 : forall m sgn ns ns' s s' u u' res res' i (H: P (SM m sgn)),
-(*   compat sgn s (RT m sgn (pc s)) -> compat sgn s' (RT m sgn (pc s')) ->  *)
   indist sgn (RT m sgn (pc s)) (RT m sgn (pc s')) s s' ->
   exec m s (inl u) -> exec m s' (inl u') ->
   region (cdr m (PM_P _ H)) i (pc u) ->
@@ -894,21 +577,10 @@ Lemma junction_indist_2 : forall m sgn ns ns' s s' u u' res res' i (H: P (SM m s
   (exists v, exists ps, 
     evalsto m ps v res /\ ps <= ns /\
     junc (cdr m (PM_P _ H)) i (pc v) /\ 
-(*     compat sgn v (RT m sgn (pc v)) /\  *)
     indist sgn (RT m sgn (pc v)) (RT m sgn (pc u')) v u').
 Proof. 
   intros.
-  (* assert (compat sgn u (RT m sgn (pc u))) as Hcompat.
-    destruct (T m sgn H).
-    Cleanexand.
-    assert (H3':=H3).
-    apply exec_step_some with (1:=PM_P _ H) in H3.
-    specialize H13 with (i:=pc s) (j:=pc u) (1:=H3).
-    destruct H13.
-    Cleanexand.
-    apply sub_compat with (rt1:=x); auto.
-    apply compat_exec_intra with (m:=m) (se:=se m sgn) (s:=s) (rt:=RT m sgn (pc s)) (H0:=H); auto. *)
-  elim evalsto_path with (1:=H3) (* (2:=Hcompat) *) (2:=H6); intros.
+  elim evalsto_path with (1:=H3) (2:=H6); intros.
   destruct H9 as [v [Hpath H9]].
   exists v.
   Cleanexand.
@@ -950,11 +622,6 @@ Definition tni :=
   indist sgn (RT m sgn (pc s)) (RT m sgn (pc s)) s s' ->
   tevalsto m (PM_P _ H) sgn (se m sgn) (RT m sgn) p s r -> 
   tevalsto m (PM_P _ H) sgn (se m sgn) (RT m sgn) p' s' r' -> 
-(*   compat sgn s (RT m sgn (pc s)) ->
-  compat sgn s' (RT m sgn (pc s')) -> *)
-(*   exists br, exists br', *)
-(*   border b br /\ *)
-(*   border b' br' /\ *)
   rindist sgn r r'.
 
 Lemma tni_ni : tni -> ni.
@@ -965,8 +632,6 @@ Proof.
   rewrite T1; auto.
   apply typable_evalsto; auto.
   apply typable_evalsto; auto.
-(*   rewrite T1 with (rt:=rt); auto.
-  rewrite T1 with (rt:=rt); auto. *)
 Qed.
 
 Variable branch_indist : forall m sgn s s' u u' (H:P (SM m sgn)), 
@@ -987,18 +652,17 @@ Proof.
   inversion Htevalsto; inversion Htevalsto'.
   (* *)
   inversion H0; inversion H4.
-  subst. (* rewrite <- Hpc in Hindist. *)
+  subst. 
   rewrite <- Hpc in H15.
-  eapply indist2_return with (1:=Hindist) (5:=H11) (6:=H15) (* (7:=H11) (8:=H15) *); auto. 
+  eapply indist2_return with (1:=Hindist) (5:=H11) (6:=H15); auto. 
   
   (* *)
-(*   inversion H0; inversion H4; subst. *)
-(*   rewrite H0 in H19. *) subst.
+  subst.
   apply tevalsto_diff_high_result with (s:=s) (res:=r) in Htevalsto'; auto.
   inversion Htevalsto'; apply high_result_indist; auto. 
   destruct n; auto. inversion H5. omega.
   (* *)
-  (* inversion H6; inversion H10;  *) subst.
+  subst.
   apply tevalsto_diff_high_result with (s:=s') (res:=r') in Htevalsto; auto.
   inversion Htevalsto; apply high_result_indist; auto.
   destruct n; auto. inversion H1. omega.
@@ -1014,12 +678,7 @@ Proof.
   apply sub_simple with (rt:=rt'0).  
   apply indist_sym. apply sub_simple with (rt:=rt'); auto.
   rewrite H2; auto. 
-(*   (* compat *)
-  apply sub_compat with rt'; auto. 
-  apply compat_exec_intra with m (se m sgn) s (RT m sgn (pc s)) H; auto.
-  rewrite Hpc; auto.
-  apply sub_compat with rt'0; auto.
-  apply compat_exec_intra with m (se m sgn) s' (RT m sgn (pc s')) H; auto. *)
+
   (* pc s <> pc s' *)
   elim (soap1 (cdr m (PM_P _ H))) with (pc s) (pc s2) (pc s3); try (rewrite Hpc; auto; fail); auto; intros.
   elim (soap1 (cdr m (PM_P _ H))) with (pc s) (pc s3) (pc s2); try (rewrite Hpc; auto; fail); auto; intros.
@@ -1050,8 +709,6 @@ Proof.
   apply Hind with (p:=n) (q:=x0) (s:=s2) (s':=x) (r:=r) (r':=r') (H:=H); auto; try omega.
   apply indist_sym; rewrite Hpcx in H10; auto.
   apply typable_evalsto; auto.  
-(*   apply compat_exec_intra with (m:=m) (se:=se m sgn) (s':=s2) (rt':=rt') (H0:=H) in H4; auto. *)
-(*   apply sub_compat with (rt1:=rt'); auto. *)
   apply indist_sym; rewrite <- Hpc; auto.
   assert ((forall j:PC, (region (cdr m (PM_P _ H)) (pc s) j) -> ~ leql (se m sgn j) observable)).
     intros. apply soap2_basic_intra with (m:=m) (sgn:=sgn) (rt:=RT m sgn (pc s)) 
@@ -1071,8 +728,6 @@ Proof.
   apply Hind with (p:=x0) (q:=n0) (s:=x) (s':=s3) (r:=r) (r':=r') (H:=H); auto; try omega.
   rewrite <- Hpcx in H10; auto.
   apply typable_evalsto; auto.  
-(*   apply compat_exec_intra with (m:=m) (se:=se m sgn) (s':=s3) (rt':=rt'0) (H0:=H) in H5; auto. *)
-(*   apply sub_compat with (rt1:=rt'0); auto. *)
   rewrite <- Hpc; auto.
   assert ((forall j:PC, (region (cdr m (PM_P _ H)) (pc s) j) -> ~ leql (se m sgn j) observable)).
     intros. apply soap2_basic_intra with (m:=m) (sgn:=sgn) (rt:=RT m sgn (pc s)) 
@@ -1088,46 +743,22 @@ Proof.
   contradiction.
   apply exec_step_some with (1:=PM_P _ H) in H16. rewrite Hpc; auto.
 Qed.
-(* 
-Theorem safe_ses : forall m sgn s r n p,
-  P (SM m sgn) ->
-  init_pc m (pc s) ->
-  compat sgn s s0 ->
-  evalsto m n p s r -> 
-  side_effect sgn s (inr _ r).
-Proof.
-  intros.
-  apply (@ses_induction n m sgn s r n p H); auto.
-  apply typable_evalsto; auto.
-  destruct (T _ _ H) as [T1 _]; rewrite T1; auto.
-Qed.
-*)
+
 Theorem safe_ni : forall m sgn p p' s s' r r',
   P (SM m sgn) ->
   init_pc m (pc s) ->
   init_pc m (pc s') ->
-(*   rt0 m sgn rt -> *)
-(*   rt0 m sgn rt -> *)
-(*   compat sgn s rt ->
-  compat sgn s' rt -> *)
   indist sgn (rt0 m sgn) (rt0 m sgn) s s' ->
   pc s = pc s' ->
   evalsto m p s r -> 
   evalsto m p' s' r' -> 
-  (* exists br, exists br',
-    border b br /\
-    border b' br' /\ *)
     rindist sgn r r'.
 Proof.
   intros.
-  apply (@ni_ind (* (max n n') *) m sgn p p' s s' r r' H); auto.
+  apply (@ni_ind m sgn p p' s s' r r' H); auto.
   destruct (T _ _ H) as [T1 _]. rewrite T1; auto.
   apply typable_evalsto; auto.
-(*   apply le_max_l. *)
   apply typable_evalsto; auto.
-(*   apply le_max_r. *)
-(*   destruct (T _ _ H) as [T1 _]; rewrite T1 with (i:=pc s) (rt:=rt); auto. *)
-(*   destruct (T _ _ H) as [T1 _]; rewrite T1 with (i:=pc s') (rt:=rt); auto. *)
 Qed.
 
 End TypableProg.
