DEX_I/DEX_BigStep.v
@@ -1,0 +1,119 @@
+(** * Bicolano: Big step (interface implementation) *)
+
+(* <Insert License Here>
+
+    $Id: BigStep.v 68 2006-02-02 15:06:27Z davidpichardie $ *)
+
+(** Big step semantics.
+
+ @author David Pichardie *)
+
+(* Hendra : - Modified to suit DEX program. 
+            - Also trim the system to contain only Arithmetic *)
+
+Require Export DEX_BigStepType.
+Require Export DEX_ImplemDomain.
+
+Open Scope type_scope.
+
+Module DEX_BigStep <: DEX_BIGSTEP.
+ 
+  Module DEX_Dom := DEX_ImplemDomain.DEX_Dom.
+ 
+  (* Inductive definition are put in BigStepLoad.v.
+     They are shared with BigStepType.v *)
+  Load "DEX_BigStepLoad.v".
+ 
+  Lemma IntraStep_ind_ : 
+      forall (p:DEX_Program) (P:DEX_Method->DEX_IntraNormalState->DEX_IntraNormalState+DEX_ReturnState->Prop),
+         (forall m s, P m s (inl _ s)) ->
+         (forall m s r, DEX_exec_return p m s r -> P m s (inr _ r)) ->
+         (forall m s s' , DEX_exec_intra p m s s' -> 
+            forall r, DEX_IntraStepStar p m s' r -> P m s' r ->
+            P m s r) ->
+      forall m s r, DEX_IntraStep p m s r -> 
+        match r with
+        | inr r' => P m s (inr _ r')
+        | inl s' => forall r', DEX_IntraStepStar p m s' r' -> P m s' r' -> P m s r'
+        end.
+     Proof.
+       intros p P H0 Hr Hi Hcr Hc.
+       fix intra 2;intros r Hs;case Hs;clear r Hs;intros.
+       apply Hr;trivial.
+       apply Hi with s2;trivial. 
+     Qed.
+
+  Lemma IntraStepStar_ind : 
+    forall (p:DEX_Program) 
+     (P : DEX_Method -> DEX_IntraNormalState -> DEX_IntraNormalState + DEX_ReturnState -> Prop),
+       (forall m s, P m s (inl _ s)) ->
+       (forall m s r, DEX_exec_return p m s r -> P m s (inr _ r)) ->
+       (forall m s s' , DEX_exec_intra p m s s' -> 
+          forall r, DEX_IntraStepStar p m s' r -> P m s' r ->
+          P m s r) ->
+    forall m s r, DEX_IntraStepStar p m s r -> P m s r.
+   Proof.
+     intros p P H0 Hr Hi.
+     fix fixp 4; intros m s' s Ht;case Ht;clear Ht s' s;intros.
+     apply H0.
+     generalize (IntraStep_ind_ p P H0 Hr Hi _ _ _ H).
+     case r;intros;trivial.
+     apply H1;trivial. constructor.
+     assert (HH:=IntraStep_ind_  p P H0 Hr Hi _ _ _ H);simpl in HH.
+     apply HH;trivial.   
+     apply fixp;trivial.
+   Qed.
+
+  Lemma IntraStepStar_intra_ind : 
+    forall (p:DEX_Program) 
+     (P : DEX_Method -> DEX_IntraNormalState -> DEX_IntraNormalState -> Prop),
+       (forall m s, P m s s) ->
+       (forall m s s', DEX_exec_intra p m s s' -> 
+          forall s'', DEX_IntraStepStar_intra p m s' s'' -> P m s' s'' ->
+          P m s s'') ->
+    forall m s s', DEX_IntraStepStar_intra p m s s' -> P m s s'.
+   Proof.
+     intros p P H0 Hi Hc.
+     assert (forall m s r, DEX_IntraStepStar p m s r ->
+              forall s', r = inl _ s' -> P m s s').
+      induction 1 using IntraStepStar_ind;intros;try discriminate;subst;eauto.
+      inversion H;auto.
+     intros; eapply H; eauto. 
+   Qed.
+
+  Lemma BigStep_ind : 
+    forall (p:DEX_Program) 
+     (P : DEX_Method -> DEX_IntraNormalState -> DEX_ReturnState -> Prop),
+       (forall m s r, DEX_exec_return p m s r -> P m s r) ->
+       (forall m s s' , DEX_exec_intra p m s s' -> 
+          forall r, DEX_BigStep p m s' r -> P m s' r ->
+          P m s r) ->
+    forall m s r, DEX_BigStep p m s r -> P m s r.
+  Proof.
+   intros p P Hr Hi Hcr Hc.
+   assert (forall m s R, DEX_IntraStepStar p m s R -> forall r, R = inr _ r -> P m s r).
+   induction 1 using IntraStepStar_ind;intros r0 Heq;try inversion Heq;subst;
+    try (eauto;fail).
+   intros;eapply H;eauto. 
+  Qed.
+
+  Lemma ReachableStar_ind : 
+    forall (p:DEX_Program) 
+     (P : (DEX_Method * DEX_IntraNormalState) -> (DEX_Method * DEX_IntraNormalState) -> Prop),
+       (forall m s, P (m,s) (m,s)) ->
+       (forall m s s', DEX_exec_intra p m s s' -> 
+          forall m' s'', ClosReflTrans (DEX_ReachableStep p) (m,s') (m',s'') -> 
+          P (m,s') (m',s'') ->
+          P (m,s) (m',s'')) ->
+    forall ms ms', 
+       ClosReflTrans (DEX_ReachableStep p) ms ms' -> P ms ms'.
+   Proof.
+     intros p P H0 Hi Hc Hsc.
+     induction 1;intros.
+     destruct a;eauto.
+     destruct a'' as (m'',s'').
+     inversion H;subst;eauto.
+     inversion H2;clear H2;subst;eauto.
+   Qed.
+
+End DEX_BigStep.
