DEX_I/DEX_BigStepLoad.v
@@ -1,0 +1,283 @@
+(* Hendra : DEX big step semantics, looking into BigStepLoad.v as reference *)
+
+  Import DEX_Dom DEX_Prog.
+
+  Open Scope type_scope.
+  Definition DEX_InitCallState :=  DEX_Method * DEX_Registers.t.
+  Definition DEX_IntraNormalState := DEX_PC * DEX_Registers.t.
+  Definition DEX_ReturnState := DEX_ReturnVal.
+
+
+  Inductive DEX_NormalStep (p:DEX_Program) : DEX_Method -> DEX_IntraNormalState -> DEX_IntraNormalState  -> Prop :=
+  | nop : forall m pc pc' regs,
+
+    instructionAt m pc = Some DEX_Nop ->
+    next m pc = Some pc' ->
+
+    DEX_NormalStep p m (pc, regs) (pc', regs)
+
+  | const : forall m pc pc' regs regs' k rt v,
+
+    instructionAt m pc = Some (DEX_Const k rt v) ->
+    In rt (DEX_Registers.dom regs) ->
+    next m pc = Some pc' ->
+    (-2^31 <= v < 2^31)%Z ->
+    DEX_METHOD.valid_reg m rt ->
+    regs' = DEX_Registers.update regs rt (Num (I (Int.const v))) ->
+
+    DEX_NormalStep p m (pc, regs) (pc', regs')
+  
+  | move_step_ok : forall m pc pc' regs regs' k rt rs v,
+
+    instructionAt m pc = Some (DEX_Move k rt rs) ->
+    In rt (DEX_Registers.dom regs) ->
+    In rs (DEX_Registers.dom regs) ->
+    next m pc = Some pc' ->
+    Some v = DEX_Registers.get regs rs ->
+    DEX_METHOD.valid_reg m rt ->
+    DEX_METHOD.valid_reg m rs ->
+    regs' = DEX_Registers.update regs rt v ->
+
+    DEX_NormalStep p m (pc, regs) (pc', regs')
+
+  | goto_step_ok : forall m pc regs o,
+
+    instructionAt m pc = Some (DEX_Goto o) ->
+
+    DEX_NormalStep p m (pc, regs) ((DEX_OFFSET.jump pc o), regs)
+(*  
+  | packedswitch_step_ok1 : forall h m pc l v r firstKey size list_offset n o,
+    
+    instructionAt m pc = Some (DEX_PackedSwitch r firstKey size list_offset) ->
+    Some (Num (I v)) = DEX_Registers.get l r ->
+    (firstKey <= Int.toZ v < firstKey + (Z_of_nat size))%Z ->
+    length list_offset = size ->
+    Z_of_nat n = ((Int.toZ v) - firstKey)%Z ->
+    nth_error list_offset n = Some o ->
+    DEX_METHOD.valid_reg m r ->
+    
+    DEX_NormalStep p m (pc, (h, l)) ((DEX_OFFSET.jump pc o), (h, l))
+
+  | packedswitch_step_ok2 : forall h m pc pc' l v r firstKey size list_offset,
+    
+    instructionAt m pc = Some (DEX_PackedSwitch r firstKey size list_offset) ->
+    Some (Num (I v)) = DEX_Registers.get l r ->
+    length list_offset = size ->
+    (Int.toZ v < firstKey \/ firstKey + (Z_of_nat size) <= Int.toZ v)%Z ->
+    next m pc = Some pc' ->
+    DEX_METHOD.valid_reg m r ->
+
+    DEX_NormalStep p m (pc, (h, l)) (pc', (h, l))
+  
+  | sparseswitch_step_ok1 : forall h m pc l v v' o r size listkey,
+    
+    instructionAt m pc = Some (DEX_SparseSwitch r size listkey) ->
+    length listkey = size ->
+    Some (Num (I v)) = DEX_Registers.get l r ->
+    List.In (pair v' o) listkey ->
+    v' = Int.toZ v ->
+    DEX_METHOD.valid_reg m r ->
+    
+    DEX_NormalStep p m (pc, (h, l)) ((DEX_OFFSET.jump pc o), (h, l))
+
+  | sparseswitch_step_ok2 : forall h m pc pc' l v r size listkey,
+
+    instructionAt m pc = Some (DEX_SparseSwitch r size listkey) ->
+    length listkey = size ->
+    Some (Num (I v)) = DEX_Registers.get l r ->
+    (forall v' o, List.In (pair v' o) listkey ->  v' <> Int.toZ v) ->
+    next m pc = Some pc' ->
+    DEX_METHOD.valid_reg m r ->
+
+    DEX_NormalStep p m (pc, (h, l)) (pc', (h, l))
+*)
+
+  | ifcmp_step_jump : forall m pc regs va vb cmp ra rb o,
+
+    instructionAt m pc = Some (DEX_Ifcmp cmp ra rb o) ->
+    In ra (DEX_Registers.dom regs) ->
+    In rb (DEX_Registers.dom regs) ->
+    Some (Num (I va)) = DEX_Registers.get regs ra ->
+    Some (Num (I vb)) = DEX_Registers.get regs rb ->
+    SemCompInt cmp (Int.toZ va) (Int.toZ vb) ->
+    DEX_METHOD.valid_reg m ra ->
+    DEX_METHOD.valid_reg m rb ->
+    
+    DEX_NormalStep p m (pc, regs) ((DEX_OFFSET.jump pc o), regs)
+
+  | ifcmp_step_continue : forall m pc pc' regs va vb cmp ra rb o,
+    
+    instructionAt m pc = Some (DEX_Ifcmp cmp ra rb o) ->
+    In ra (DEX_Registers.dom regs) ->
+    In rb (DEX_Registers.dom regs) ->
+    Some (Num (I va)) = DEX_Registers.get regs ra ->
+    Some (Num (I vb)) = DEX_Registers.get regs rb ->
+    ~SemCompInt cmp (Int.toZ va) (Int.toZ vb) ->
+    next m pc = Some pc' ->
+    DEX_METHOD.valid_reg m ra ->
+    DEX_METHOD.valid_reg m rb ->
+
+    DEX_NormalStep p m (pc, regs) (pc', regs)
+
+  | ifz_step_jump : forall m pc regs v cmp r o,
+
+    instructionAt m pc = Some (DEX_Ifz cmp r o) ->
+    In r (DEX_Registers.dom regs) ->
+    Some (Num (I v)) = DEX_Registers.get regs r ->
+    SemCompInt cmp (Int.toZ v) (0) ->
+    DEX_METHOD.valid_reg m r ->
+    
+    DEX_NormalStep p m (pc, regs) ((DEX_OFFSET.jump pc o), regs)
+
+  | ifz_step_continue : forall m pc pc' regs v cmp r o,
+    
+    instructionAt m pc = Some (DEX_Ifz cmp r o) ->
+    In r (DEX_Registers.dom regs) ->
+    Some (Num (I v)) = DEX_Registers.get regs r ->
+    ~SemCompInt cmp (Int.toZ v) (0) ->
+    next m pc = Some pc' ->
+
+    DEX_NormalStep p m (pc, regs) (pc', regs)
+
+  (** <addlink>ineg</addlink>: Negate [int] *)
+  | ineg_step : forall m pc regs regs' pc' rt rs v,
+
+    instructionAt m pc = Some (DEX_Ineg rt rs) ->
+    In rt (DEX_Registers.dom regs) ->
+    In rs (DEX_Registers.dom regs) ->
+    next m pc = Some pc' ->
+    Some (Num (I v)) = DEX_Registers.get regs rs ->
+    DEX_METHOD.valid_reg m rt ->
+    DEX_METHOD.valid_reg m rs ->
+    regs' = DEX_Registers.update regs rt (Num (I (Int.neg v))) ->
+
+    DEX_NormalStep p m (pc, regs) (pc', regs')
+
+  (** <addlink>ineg</addlink>: Not [int] (one's complement) *)
+  | inot_step : forall (*h*) m pc regs regs' pc' rt rs v,
+
+    instructionAt m pc = Some (DEX_Inot rt rs) ->
+    In rt (DEX_Registers.dom regs) ->
+    In rs (DEX_Registers.dom regs) ->
+    next m pc = Some pc' ->
+    Some (Num (I v)) = DEX_Registers.get regs rs ->
+    DEX_METHOD.valid_reg m rt ->
+    DEX_METHOD.valid_reg m rs ->
+    regs' = DEX_Registers.update regs rt (Num (I (Int.not v))) ->
+
+    DEX_NormalStep p m (pc, regs) (pc', regs')
+
+  (** <addlink>i2b</addlink>: Convert [int] to [byte] *)
+  | i2b_step_ok : forall m pc pc' regs regs' rt rs v,
+
+    instructionAt m pc = Some (DEX_I2b rt rs) ->
+    In rt (DEX_Registers.dom regs) ->
+    In rs (DEX_Registers.dom regs) ->
+    next m pc = Some pc' ->
+    Some (Num (I v)) = DEX_Registers.get regs rs ->
+    DEX_METHOD.valid_reg m rt ->
+    DEX_METHOD.valid_reg m rs ->
+    regs' = DEX_Registers.update regs rt (Num (I (b2i (i2b v)))) ->
+    
+    DEX_NormalStep p m (pc, regs) (pc', regs')
+
+ (** <addlink>i2s</addlink>: Convert [int] to [short] *)
+  | i2s_step_ok : forall m pc pc' regs regs' rt rs v,
+
+    instructionAt m pc = Some (DEX_I2s rt rs) ->
+    In rt (DEX_Registers.dom regs) ->
+    In rs (DEX_Registers.dom regs) ->
+    next m pc = Some pc' ->
+    Some (Num (I v)) = DEX_Registers.get regs rs ->
+    DEX_METHOD.valid_reg m rt ->
+    DEX_METHOD.valid_reg m rs ->
+    regs' = DEX_Registers.update regs rt (Num (I (s2i (i2s v)))) ->
+
+    DEX_NormalStep p m (pc, regs) (pc', regs')
+
+  | ibinop_step_ok : forall m pc pc' regs regs' op rt ra rb va vb,
+
+    instructionAt m pc = Some (DEX_Ibinop op rt ra rb) ->
+    In rt (DEX_Registers.dom regs) ->
+    In ra (DEX_Registers.dom regs) ->
+    In rb (DEX_Registers.dom regs) ->
+    next m pc = Some pc' ->
+    (*(op = DivInt \/ op = RemInt -> ~ Int.toZ i2 = 0) -> at this moment there is no exception*)
+    Some (Num (I va)) = DEX_Registers.get regs ra ->
+    Some (Num (I vb)) = DEX_Registers.get regs rb ->
+    DEX_METHOD.valid_reg m rt ->
+    DEX_METHOD.valid_reg m ra ->
+    DEX_METHOD.valid_reg m rb ->
+    regs' = DEX_Registers.update regs rt (Num (I (SemBinopInt op va vb))) ->
+
+    DEX_NormalStep p m (pc, regs) (pc', regs')
+
+  | ibinopconst_step_ok : forall m pc pc' regs regs' op rt r va v,
+
+    instructionAt m pc = Some (DEX_IbinopConst op rt r v) ->
+    In r (DEX_Registers.dom regs) ->
+    In rt (DEX_Registers.dom regs) ->
+    next m pc = Some pc' ->
+    (*(op = DivInt \/ op = RemInt -> ~ Int.toZ i2 = 0) -> at this moment there is no exception*)
+    Some (Num (I va)) = DEX_Registers.get regs r ->
+    DEX_METHOD.valid_reg m rt ->
+    DEX_METHOD.valid_reg m r ->
+    regs' = DEX_Registers.update regs rt (Num (I (SemBinopInt op va (Int.const v)))) ->
+
+    DEX_NormalStep p m (pc, regs) (pc', regs')
+.
+
+  Inductive DEX_ReturnStep (p:DEX_Program) : DEX_Method -> DEX_IntraNormalState -> DEX_ReturnState -> Prop :=
+  | void_return : forall m pc regs,
+
+    instructionAt m pc = Some DEX_Return -> 
+    DEX_METHODSIGNATURE.result (DEX_METHOD.signature m) = None ->
+
+    DEX_ReturnStep p m (pc, regs) (Normal None)
+
+  | vreturn : forall m pc regs val t k rs,
+    (* Implicit in the assumption is that the register has a value in it *)
+    instructionAt m pc = Some (DEX_VReturn k rs) ->
+    In rs (DEX_Registers.dom regs) ->
+    DEX_METHODSIGNATURE.result (DEX_METHOD.signature m) = Some t ->
+    assign_compatible p val t ->
+    compat_ValKind_value k val ->
+    Some val = DEX_Registers.get regs rs ->
+
+    DEX_ReturnStep p m (pc, regs) (Normal (Some val))
+.
+
+  Inductive DEX_exec_intra (p:DEX_Program) (m:DEX_Method) : DEX_IntraNormalState -> DEX_IntraNormalState -> Prop :=
+  | exec_intra_normal : forall s1 s2,
+     DEX_NormalStep p m s1 s2 ->
+     DEX_exec_intra p m s1 s2.
+
+  Inductive DEX_exec_return (p:DEX_Program) (m:DEX_Method) : DEX_IntraNormalState -> DEX_ReturnState -> Prop :=
+  | exec_return_normal : forall s ov,
+     DEX_ReturnStep p m s (Normal ov) ->
+     DEX_exec_return p m s (Normal ov)
+.
+
+ Inductive DEX_IntraStep (p:DEX_Program) : 
+    DEX_Method -> DEX_IntraNormalState -> DEX_IntraNormalState + DEX_ReturnState -> Prop :=
+  | IntraStep_res :forall m s ret,
+     DEX_exec_return p m s ret ->
+     DEX_IntraStep p m s (inr _ ret)
+  | IntraStep_intra_step:forall m s1 s2,
+     DEX_exec_intra p m s1 s2 ->
+     DEX_IntraStep p m s1 (inl _ s2) .
+ 
+ Definition DEX_IntraStepStar p m s r := TransStep_l (DEX_IntraStep p m) s r.
+
+ Definition DEX_IntraStepStar_intra p m s s' := DEX_IntraStepStar p m s (inl _ s').
+
+ Definition DEX_BigStep  p m s ret := DEX_IntraStepStar p m s (inr _ ret).
+
+ Inductive DEX_ReachableStep (P:DEX_Program) : 
+      (DEX_Method*DEX_IntraNormalState)->(DEX_Method*DEX_IntraNormalState) ->Prop :=
+   | ReachableIntra : forall M s s', 
+       DEX_IntraStep P M s (inl _ s') ->
+       DEX_ReachableStep P (M,s) (M,s').
+
+ Definition DEX_Reachable P M s s' := 
+   exists M',  ClosReflTrans (DEX_ReachableStep P) (M,s) (M',s').
