DEX_I/DEX_BigStepType.v
@@ -1,0 +1,98 @@
+(** * Bicolano: Big step (interface only) *)
+
+(* <Insert License Here>
+
+    $Id: BigStep.v 68 2006-02-02 15:06:27Z davidpichardie $ *)
+
+(** Big step semantics.
+
+ @author Benjamin Gregoire *)
+(* Hendra : - Modified to suit DEX program. 
+            - Also trim the system to contain only Arithmetic *)
+
+Require Export DEX_Domain.
+
+Set Implicit Arguments.
+Definition cons_option (A:Set) (o:option A) (l:list A) := 
+   match o with 
+   | None => l
+   | Some e => e::l
+   end.
+Unset Implicit Arguments.
+
+Section TRANS.
+ Set Implicit Arguments.
+ Variable A B :Type.
+ Variable R : A -> A + B -> Prop.
+
+ Inductive TransStep_l : A -> A + B -> Prop :=
+   | TransStep_l_refl : forall a,
+       TransStep_l a (inl _ a)
+   | TransStep_l_one : forall a r,
+        R a r -> TransStep_l a r
+   | TransStep_l_trans : forall a1 a2 r,
+       R a1 (inl _ a2) -> 
+       TransStep_l a2 r ->
+       TransStep_l a1 r.
+
+ Variable R' : A -> A -> Prop.
+
+ Inductive ClosReflTrans : A -> A -> Prop :=
+   | ClosReflTrans_refl : forall a, ClosReflTrans a a
+   | ClosReflTrans_trans : forall a a' a'',
+       R' a a' ->
+       ClosReflTrans a' a'' ->
+       ClosReflTrans a a''.
+
+ Unset Implicit Arguments.
+
+End TRANS.
+
+Open Scope type_scope.
+
+Module Type DEX_BIGSTEP.
+
+ Declare Module DEX_Dom : DEX_SEMANTIC_DOMAIN.
+
+ Load "DEX_BigStepLoad.v".
+
+  Parameter IntraStepStar_ind : 
+   forall (p:DEX_Program) 
+    (P : DEX_Method -> DEX_IntraNormalState -> DEX_IntraNormalState + DEX_ReturnState -> Prop),
+      (forall m s, P m s (inl _ s)) ->
+      (forall m s r, DEX_exec_return p m s r -> P m s (inr _ r)) ->
+      (forall m s s' , DEX_exec_intra p m s s' -> 
+         forall r, DEX_IntraStepStar p m s' r -> P m s' r ->
+         P m s r) ->
+   forall m s r, DEX_IntraStepStar p m s r -> P m s r.
+
+  Parameter IntraStepStar_intra_ind : 
+   forall (p:DEX_Program) 
+    (P : DEX_Method -> DEX_IntraNormalState -> DEX_IntraNormalState -> Prop),
+      (forall m s, P m s s) ->
+      (forall m s s', DEX_exec_intra p m s s' -> 
+         forall s'', DEX_IntraStepStar_intra p m s' s'' -> P m s' s'' ->
+         P m s s'') ->
+   forall m s s', DEX_IntraStepStar_intra p m s s' -> P m s s'.
+  
+  Parameter BigStep_ind : 
+   forall (p:DEX_Program) 
+    (P : DEX_Method -> DEX_IntraNormalState -> DEX_ReturnState -> Prop),
+      (forall m s r, DEX_exec_return p m s r -> P m s r) ->
+      (forall m s s' , DEX_exec_intra p m s s' -> 
+         forall r, DEX_BigStep p m s' r -> P m s' r ->
+         P m s r) ->
+   forall m s r, DEX_BigStep p m s r -> P m s r.
+
+  Parameter ReachableStar_ind : 
+   forall (p:DEX_Program) 
+    (P : (DEX_Method * DEX_IntraNormalState) -> (DEX_Method * DEX_IntraNormalState) -> Prop),
+      (forall m s, P (m,s) (m,s)) ->
+      (forall m s s', DEX_exec_intra p m s s' -> 
+         forall m' s'', ClosReflTrans (DEX_ReachableStep p) (m,s') (m',s'') -> 
+         P (m,s') (m',s'') ->
+         P (m,s) (m',s'')) ->
+   forall ms ms', 
+      ClosReflTrans (DEX_ReachableStep p) ms ms' -> P ms ms'.
+
+End DEX_BIGSTEP.
