DEX_I/DEX_ElemLemmaNormalIntra3.v
@@ -1,0 +1,78 @@
+Require Export DEX_ElemLemmas.
+
+Import DEX_BigStepWithTypes.DEX_BigStepWithTypes DEX_BigStep.DEX_Dom DEX_Prog.
+
+Section p.
+
+Variable kobs: L.t.
+Variable p:DEX_ExtendedProgram.
+Variable se : DEX_PC -> L.t.
+Variable reg : DEX_PC -> DEX_PC -> Prop.
+Variable m : DEX_Method.
+
+Ltac soap2_intra_normal_aux Hreg_in H Hreg r lvl Hget_ori Hvalue_opt_in k k':=
+  specialize Hreg_in with r;
+  inversion Hreg_in as [k k' Hget Hget' Hleq Hleq'| Hvalue_opt_in];
+  try (apply H in Hreg; apply leql_join_each in Hreg; inversion Hreg as [Hleql1 Hleql1'];
+    apply not_leql_trans with (k2:=lvl) in Hleq; auto);
+  try (apply H in Hreg; apply not_leql_trans with (k2:=lvl) in Hleq; auto);
+  try (rewrite Hget in Hget_ori; inversion Hget_ori; subst; auto).
+
+(* High Branching *)
+Lemma soap2_intra_normal : 
+ forall sgn pc pc2 pc2' i r1 rt1 r1' rt1' r2 r2' rt2 rt2' ,
+   instructionAt m pc = Some i ->
+   NormalStep se reg m sgn i (pc,r1) rt1 (pc2,r2) rt2 ->
+   NormalStep se reg m sgn i (pc,r1') rt1' (pc2',r2') rt2' ->
+   pc2 <> pc2' ->
+   st_in kobs rt1 rt1' (pc,r1) (pc,r1') ->
+
+    forall j, reg pc j -> ~ L.leql (se j) kobs.
+Proof.
+  intros sgn pc pc2 pc2' i r1 rt1 r1' rt1' r2 r2' rt2 rt2' Hins Hstep Hstep' Hpc Hst_in j Hreg.
+  destruct i; simpl in Hins, Hstep, Hstep', Hst_in; 
+  inversion_clear Hstep in Hins Hstep' Hpc Hst_in;
+  inversion_clear Hstep' in Hpc Hst_in; subst;
+  apply inv_st_in in Hst_in;
+  DiscrimateEq; try (elim Hpc; reflexivity); try (contradiction).
+  (* If_icmp *)
+  inversion Hst_in as [Heqset Hreg_in].
+    (* ra *)
+    assert (Hreg_in':=Hreg_in).
+    soap2_intra_normal_aux Hreg_in H8 Hreg ra (se j) H5 Hvalue_opt_in k k'.
+    (* rb *)
+    soap2_intra_normal_aux Hreg_in' H8 Hreg rb (se j) H6 Hvalue_opt_in' k k'.
+    (* both are low *)
+    rewrite <- H3 in Hvalue_opt_in; rewrite <- H4 in Hvalue_opt_in'; 
+    rewrite <- H14 in Hvalue_opt_in; rewrite <- H15 in Hvalue_opt_in'.
+    inversion Hvalue_opt_in as [v v' Hvalue_in | Hnone]; 
+    inversion Hvalue_opt_in' as [v2 v2' Hvalue_in' | Hnone'];
+    inversion Hvalue_in; inversion Hvalue_in'. 
+    subst; contradiction.  
+  inversion Hst_in as [Heqset Hreg_in].
+    (* ra *)
+    assert (Hreg_in':=Hreg_in).
+    soap2_intra_normal_aux Hreg_in H9 Hreg ra (se j) H6 Hvalue_opt_in k k'.
+    (* rb *)
+    soap2_intra_normal_aux Hreg_in' H9 Hreg rb (se j) H7 Hvalue_opt_in' k k'.
+    (* both are low *)
+    rewrite <- H4 in Hvalue_opt_in; rewrite <- H5 in Hvalue_opt_in'; 
+    rewrite <- H14 in Hvalue_opt_in; rewrite <- H15 in Hvalue_opt_in'.
+    inversion Hvalue_opt_in as [v v' Hvalue_in | Hnone]; 
+    inversion Hvalue_opt_in' as [v2 v2' Hvalue_in' | Hnone'];
+    inversion Hvalue_in; inversion Hvalue_in'. 
+    subst; contradiction.   
+  (* If_z *)
+  inversion Hst_in as [Heq_set Hreg_in].
+    soap2_intra_normal_aux Hreg_in H4 Hreg r (se j) H2 Hvalue_opt_in k1 k1'.
+    rewrite <- H1 in Hvalue_opt_in; rewrite <- H8 in Hvalue_opt_in;
+      inversion Hvalue_opt_in as [v v' Hvalue_in | Hnone]; 
+      inversion Hvalue_in; subst; contradiction.
+  inversion Hst_in as [Heq_set Hreg_in].
+    soap2_intra_normal_aux Hreg_in H5 Hreg r (se j) H3 Hvalue_opt_in k1 k1'.
+    rewrite <- H2 in Hvalue_opt_in; rewrite <- H8 in Hvalue_opt_in;
+      inversion Hvalue_opt_in as [v v' Hvalue_in | Hnone]; 
+      inversion Hvalue_in; subst; contradiction.
+Qed. 
+
+End p.
