DEX_I/DEX_ElemLemmas.v
@@ -1,0 +1,72 @@
+Require Export DEX_BigStepWithTypes.
+
+Import DEX_BigStepWithTypes DEX_BigStepAnnot.DEX_BigStepAnnot 
+  DEX_BigStep.DEX_BigStep DEX_Dom DEX_Prog.
+
+
+Lemma reduce_dec_true : forall (P:Prop) (test:{P}+{~P}),
+   P -> exists h, test = left (~P) h.
+Proof.
+  intros.
+  destruct test; contradiction || eauto.
+Qed.
+
+Lemma reduce_dec_false : forall (P:Prop) (test:{P}+{~P}),
+   ~P -> exists h, test = right P h.
+Proof.
+  intros.
+  destruct test; contradiction || eauto.
+Qed.
+
+Ltac reduce_leql_dec :=
+  match goal with
+   [ id : ~ L.leql ?x ?y |- context[L.leql_dec ?x ?y] ] => 
+      let h := fresh "h" in
+      let Heq := fresh "Heq" in 
+        (destruct (reduce_dec_false _ (L.leql_dec x y) id) as [h Heq];
+          simpl in Heq;
+         rewrite Heq; clear h Heq)
+  |[ id : L.leql ?x ?y |- context[L.leql_dec ?x ?y] ] => 
+      let h := fresh "h" in
+      let Heq := fresh "Heq" in 
+        (destruct (reduce_dec_true _ (L.leql_dec x y) id) as [h Heq];
+          simpl in Heq;
+         rewrite Heq; clear h Heq)
+  end.
+
+Ltac reduce_leql_dec_strong :=
+  match goal with
+   [ id : ~ L.leql ?x ?y |- context[L.leql_dec ?x ?y] ] => 
+      let h := fresh "h" in
+      let Heq := fresh "Heq" in 
+        (destruct (reduce_dec_false _ (L.leql_dec x y) id) as [h Heq];
+         rewrite Heq; clear h Heq)
+  |[ id : L.leql ?x ?y |- context[L.leql_dec ?x ?y] ] => 
+      let h := fresh "h" in
+      let Heq := fresh "Heq" in 
+        (destruct (reduce_dec_true _ (L.leql_dec x y) id) as [h Heq];
+         rewrite Heq; clear h Heq)
+  |[ |- context[L.leql_dec ?x ?y] ] => 
+      let id := fresh in (
+      try (assert (id:L.leql x y); 
+           [simpl in *; eauto with lattice;fail
+           |let h := fresh "h" in
+            let Heq := fresh "Heq" in 
+            (destruct (reduce_dec_true _ (L.leql_dec x y) id) as [h Heq];
+             rewrite Heq; clear h Heq)]);
+      try (assert (id:~L.leql x y); 
+           [simpl in *; eauto with lattice;fail
+           |let h := fresh "h" in
+            let Heq := fresh "Heq" in 
+            (destruct (reduce_dec_false _ (L.leql_dec x y) id) as [h Heq];
+             rewrite Heq; clear h Heq)]))
+  end.
+
+Lemma inv_st_in : forall kobs pc0 pc1 r0 r1 rt0 rt1,
+ st_in kobs rt1 rt0 (pc1, r1) (pc0, r0) ->
+   Regs_in kobs r1 r0 rt1 rt0.
+Proof.
+  intros.
+  inversion_clear H; intuition.
+Qed.
+Implicit Arguments inv_st_in.
