DEX_I/DEX_ProofBigStepWithType.v
@@ -1,0 +1,70 @@
+Require Export DEX_typing_rules.
+Require Export DEX_BigStepWithTypes.
+Import  DEX_BigStep.DEX_BigStep DEX_BigStepWithTypes.DEX_BigStepWithTypes DEX_Dom DEX_Prog.
+
+Section p.
+  Variable p : DEX_ExtendedProgram.
+
+Hint Resolve L.join_least L.join_right L.join_left L.leql_trans L.leql_refl : lat.
+
+Lemma join_sym : forall a b, L.join a b = L.join b a. intros. destruct a, b; auto. Qed.
+
+Lemma well_types_imply_exec_return : forall se region m sgn i s1 rt1 rv2 ,
+     DEX_BigStepAnnot.DEX_exec_return p m s1 rv2 -> 
+     instructionAt m (fst s1) = Some i ->
+     DEX_typing_rules.texec sgn region se (fst s1) i rt1 None ->
+      exec_return p se m sgn i s1 rt1 rv2.
+Proof.
+  intros se region m sgn i s1 rt1 rv2 He.
+  inversion_clear He; intros. 
+  constructor.
+  inversion_mine H; simpl in H0; DiscrimateEq; inversion_mine H1.
+  constructor; auto. 
+  constructor 2 with t k_r kv; auto.
+  simpl in H11. 
+  rewrite join_sym in H13; auto.
+Qed.
+
+Lemma well_types_imply_NormalStep : forall se region m sgn i s1 rt1 s2 rt2,
+     DEX_BigStep.DEX_NormalStep p m s1 s2  ->
+     instructionAt m (fst s1) = Some i ->
+     texec sgn region se (fst s1) i rt1 (Some rt2) ->
+       NormalStep se region m sgn i s1 rt1 s2 rt2.
+Proof.
+  intros se region m sgn i s1 rt1 s2 t2 H.
+  inversion_clear H; simpl; intros Hi Ht; 
+  DiscrimateEq; 
+  unfold NormalStep;
+  inversion_mine Ht;
+    try (constructor;auto). 
+  (* Move *) constructor 1 with (val := v) (k:=k_rs); auto. rewrite join_sym; auto.
+  (* Ifcmp *) 
+  constructor 1 with (i1:=va) (i2:=vb) (k1:=ka) (k2:=kb); auto. 
+  constructor 2 with (i1:=va) (i2:=vb) (k1:=ka) (k2:=kb); auto.
+  (* Ifz *)
+  constructor 1 with (i:=v) (k:=k); auto. 
+  constructor 2 with (i:=v) (k:=k); auto.
+  (* Ineg *) constructor 1 with (v:=v) (k:=ks); auto. rewrite join_sym; auto.
+  (* Inot *) constructor 1 with (v:=v) (k:=ks); auto. rewrite join_sym; auto.
+  (* I2b *) constructor 1 with (v:=v) (k:=ks); auto. rewrite join_sym; auto.
+  (* I2s *) constructor 1 with (v:=v) (k:=ks); auto. rewrite join_sym; auto.
+  (* Ibinop *) constructor 1 with (i1:=va) (i2:=vb) (k1:=ka) (k2:=kb); auto. 
+    assert (forall a b c, L.join (L.join a b) (c) = L.join a (L.join b c)).
+      intros; destruct a,b,c; auto.
+    rewrite H; auto.
+  (* IbinopConst *) constructor 1 with (i:=va) (k:=ks); auto.
+Qed.
+
+Lemma well_types_imply_exec_intra : forall se region m sgn i s1 rt1 s2 rt2,
+     DEX_BigStepAnnot.DEX_exec_intra p m s1 s2  -> 
+     instructionAt m (fst s1) = Some i ->
+     texec sgn region se (fst s1) i rt1 (Some rt2) ->
+       exec_intra se region m sgn i s1 rt1 s2 rt2.
+Proof.
+  intros se region m sgn i s1 rt1 s2 rt2 He.
+  inversion_clear He; intros. 
+  constructor; auto.
+  apply well_types_imply_NormalStep; auto.
+Qed.
+
+End p.
