DEX_I/DEX_step.v
@@ -1,0 +1,347 @@
+(** Static Intra-method control flow step. We also implement an iterator on it *)
+(* Hendra : - Modified to suit DEX program. 
+            - DEX has different instructions list from JVM.
+            - Also trim the system to contain only Arithmetic
+            - Only retain the for_all_steps lemma *)
+Require Export Annotated.
+Import DEX_BigStep.DEX_Dom DEX_Prog.
+
+  Section DEX_S_section.   (** step relation **)
+    Variable m : DEX_Method.
+
+    Inductive DEX_step : DEX_PC -> DEX_Instruction -> option DEX_PC -> Prop := 
+    | DEX_nop : forall i j,
+
+      next m i = Some j ->
+      DEX_step i DEX_Nop (Some j)
+
+    | DEX_move : forall i j (k:DEX_ValKind) (rt:DEX_Reg) (rs:DEX_Reg),
+      
+      next m i = Some j ->
+      DEX_step i (DEX_Move k rt rs) (Some j)
+
+    | DEX_return_s : forall i,
+      DEX_step i DEX_Return None
+
+    | DEX_vReturn : forall i (k:DEX_ValKind) (rt:DEX_Reg),
+      DEX_step i (DEX_VReturn k rt) None
+
+    | DEX_const : forall i j (k:DEX_ValKind) (rt:DEX_Reg) (v:Z),
+
+      next m i = Some j ->
+      DEX_step i (DEX_Const k rt v) (Some j)
+
+    | DEX_goto : forall i (o:DEX_OFFSET.t),
+      DEX_step i (DEX_Goto o) (Some (DEX_OFFSET.jump i o))
+(* still experimental for PackedSwitch in that the next instruction is
+   defined as the difference between i and j *)
+(*    | packedSwitch : forall i j (rt:DEX_Reg) (firstKey:Z) (size:Z) (l:list OFFSET.t),
+      (* next m i = Some j \/ In o ((j - i)::l) -> *)
+      next m i = Some j \/ In j (@map _ _ (OFFSET.jump i) l) ->
+      step i (PackedSwitch rt firstKey size l) None (Some j)
+    | sparseSwitch : forall i j (rt:DEX_Reg) (size:Z) (l:list (Z * OFFSET.t)),
+      next m i = Some j \/ In j (@map _ _ (OFFSET.jump i) (@map _ _ (@snd _ _) l)) ->
+      step i (SparseSwitch rt size l) None (Some j) *)
+
+    | DEX_ifcmp : forall i j (cmp:DEX_CompInt) (ra:DEX_Reg) (rb:DEX_Reg) (o:DEX_OFFSET.t),
+      next m i = Some j \/ j = DEX_OFFSET.jump i o ->
+      DEX_step i (DEX_Ifcmp cmp ra rb o) (Some j)
+
+    | DEX_ifz : forall i j (cmp:DEX_CompInt) (r:DEX_Reg) (o:DEX_OFFSET.t),
+      next m i = Some j \/ j = DEX_OFFSET.jump i o ->
+      DEX_step i (DEX_Ifz cmp r o) (Some j)
+
+    | DEX_ineg : forall i j (rt:DEX_Reg) (rs:DEX_Reg),
+      next m i = Some j ->
+      DEX_step i (DEX_Ineg rt rs) (Some j)
+
+    | DEX_inot : forall i j (rt:DEX_Reg) (rs:DEX_Reg),
+      next m i = Some j ->
+      DEX_step i (DEX_Inot rt rs) (Some j)
+
+    | DEX_i2b : forall i j (rt:DEX_Reg) (rs:DEX_Reg),
+      next m i = Some j ->
+      DEX_step i (DEX_I2b rt rs) (Some j)
+
+    | DEX_i2s : forall i j (rt:DEX_Reg) (rs:DEX_Reg),
+       next m i = Some j -> 
+      DEX_step i (DEX_I2s rt rs) (Some j)
+    | DEX_ibinop : forall i j (op:DEX_BinopInt) (rt:DEX_Reg) (ra:DEX_Reg) (rb:DEX_Reg),
+       next m i = Some j -> 
+      DEX_step i (DEX_Ibinop op rt ra rb) (Some j)
+
+    | DEX_ibinopConst : forall i j (op:DEX_BinopInt) (rt:DEX_Reg) (r:DEX_Reg) (v:Z),
+       next m i = Some j -> 
+      DEX_step i (DEX_IbinopConst op rt r v) (Some j)
+(* Hendra 11082016 focus on DEX I
+    | DEX_packedSwitch : forall i j (rt:DEX_Reg) (firstKey:Z) (size:nat) (l:list DEX_OFFSET.t),
+      (*(next m i = Some d /\ d = DEX_OFFSET.jump i j) \/ In j l ->*)
+      (*(nextAddress i = Some d /\ d = jump_label i j) \/ In j l -> *)
+      (exists d, nextAddress i = Some d /\ d = jump_label i j) \/ In j l ->
+      (*DEX_step i (DEX_PackedSwitch rt firstKey size l) None (Some (DEX_OFFSET.jump i j))*)
+      DEX_step i (DEX_PackedSwitch rt firstKey size l) None (Some (jump_label i j))
+    | DEX_sparseSwitch : forall i j (rt:DEX_Reg) (size:nat) (l:list (Z * DEX_OFFSET.t)),
+      (*(next m i = Some d /\ d = DEX_OFFSET.jump i j) \/ *)
+      (exists d, nextAddress i = Some d /\ d = jump_label i j) \/ 
+        In j (@map _ _ (@snd _ _) l) ->
+      (*DEX_step i (DEX_SparseSwitch rt size l) None (Some (DEX_OFFSET.jump i j))*)
+      DEX_step i (DEX_SparseSwitch rt size l) None (Some (jump_label i j))
+*)
+.
+
+    Definition get_steps (i:DEX_PC) (ins:DEX_Instruction) (next:option DEX_PC): list (option DEX_PC) := 
+      match ins with
+(* Hendra 11082016 focus on DEX I
+        | DEX_SparseSwitch r size l =>
+          (*(None,next) :: map (fun o => (None,Some (DEX_OFFSET.jump i o))) (@map _ _ (@snd _ _) l)*)
+          (None,next) :: map (fun o => ((None:DEX_tag),Some (jump_label i o))) (@map _ _ (@snd _ _) l)
+        | DEX_PackedSwitch r firstKey size l =>
+          (*(None,next) :: map (fun o => (None,Some (DEX_OFFSET.jump i o))) (l)*)
+          (None,next) :: map (fun o => ((None:DEX_tag),(Some (jump_label i o):option address))) (l)
+*)
+        | DEX_Return => None::nil
+        | DEX_VReturn k rt => None::nil
+        | DEX_Goto o => (Some (DEX_OFFSET.jump i o))::nil
+        | DEX_Ifcmp cmp ra rb o => next::(Some (DEX_OFFSET.jump i o))::nil
+        | DEX_Ifz cmp r o => next::(Some (DEX_OFFSET.jump i o))::nil
+        | _ => next::nil
+      end.
+
+    Lemma all_step_in_get_steps : forall i ins oj,
+        DEX_step i ins oj -> 
+        In oj (get_steps i ins (next m i)).
+    Proof.
+      intros.
+      inversion_clear H;
+      simpl get_steps; try rewrite H0;
+      auto with datatypes;
+      (* ifcmp and ifz cases *)
+        try (destruct H0 as [H0|H0]; rewrite <- H0; auto with datatypes;
+        right; subst; left; reflexivity).
+      (* Hendra 11082016 focus on DEX I
+      (* PackedSwitch case *)
+        (* default case : next instruction *)
+        destruct H0. left. inversion H. inversion H0. rewrite H1. rewrite <- H2. reflexivity.
+        (* other successors case *)
+        right. try match goal with
+          [ |- In (_,_) (map ?F _) ] => 
+          apply in_map with (f:=F); try assumption
+        end. 
+      (* SparseSwitch case *)
+        (* default case : next instruction *)
+        destruct H0. left. inversion H. inversion H0. rewrite H1. rewrite <- H2. reflexivity.
+        (* other successors case *)
+        right. try match goal with
+          [ |- In (_,_) (map ?F _) ] => 
+          apply in_map with (f:=F); try assumption
+        end.
+*)
+    Qed.
+
+  Section for_all_steps.
+    Variable test : DEX_PC -> DEX_Instruction -> option DEX_PC -> bool.
+
+    Definition for_all_steps_bm (bm:DEX_BytecodeMethod) : bool :=
+      MapN.for_all _
+      (fun i (ins_next:DEX_Instruction*(option DEX_PC *list DEX_ClassName )) =>
+        let (ins,next) := ins_next in
+          for_all _
+          (fun (oj:option DEX_PC) => test i ins oj)
+          (get_steps i ins ( fst  next)))
+      bm.(DEX_BYTECODEMETHOD.instr).
+
+    Lemma for_all_steps_bm_true : forall bm,
+      DEX_METHOD.body m = Some bm ->
+      for_all_steps_bm bm = true ->
+      forall i ins oj,
+        instructionAt m i = Some ins ->
+        DEX_step i ins oj -> test i ins oj = true.
+    Proof.
+      intros.
+      assert (T1:=MapN.for_all_true _ _ _ H0).
+      assert (T2:=all_step_in_get_steps _ _ _ H2).
+      unfold instructionAt, DEX_BYTECODEMETHOD.instructionAt in H1.
+      rewrite H in H1.
+      caseeq (MapN.get (DEX_Instruction * (option DEX_PC*list DEX_ClassName)) (DEX_BYTECODEMETHOD.instr bm) i).
+      intros (ins0,next0) T3.
+      rewrite T3 in H1.
+      generalize (T1 _ _ T3); clear T1; intros T1.
+      apply for_all_true with
+        (test:=(fun oj : option DEX_PC => test i ins oj))
+        (2:=T2).
+      unfold next, DEX_BYTECODEMETHOD.nextAddress.
+      rewrite H; rewrite T3; simpl.
+      inversion_mine H1; auto.
+      intros T3; rewrite T3 in H1; discriminate.
+    Qed.
+
+  Definition for_all_steps_m : bool :=
+    match DEX_METHOD.body m with
+      | None => false
+      | Some bm => for_all_steps_bm bm
+    end.
+
+  Definition test_all_steps_m : list (DEX_PC*bool) :=
+    match DEX_METHOD.body m with
+      | None => nil
+      | Some bm => 
+      List.map
+      (fun (ins_next:DEX_PC*(DEX_Instruction*(option DEX_PC*list DEX_ClassName))) =>
+        let (i,ins_next) := ins_next in
+        let (ins,next) := ins_next in
+          (i,for_all _
+            (fun (oj:option DEX_PC) => test i ins oj)
+            (get_steps i ins (fst next))))
+      (MapN.elements _ bm.(DEX_BYTECODEMETHOD.instr))
+    end.
+
+  Lemma for_all_steps_m_true : for_all_steps_m = true ->
+      forall i ins oj,
+        instructionAt m i = Some ins ->
+        DEX_step i ins oj -> test i ins oj = true.
+  Proof.
+    unfold for_all_steps_m.
+    generalize for_all_steps_bm_true.
+    destruct (DEX_METHOD.body m) as [bm|]; intro.
+    apply H; auto.
+    intros; discriminate.
+  Qed.
+  End for_all_steps.
+
+  Section for_all_succs.
+    Variable pc:DEX_PC.
+    Variable test : option DEX_PC -> bool.
+
+    Definition for_all_succs_bm (bm:DEX_BytecodeMethod) : bool :=
+      match MapN.get _ bm.(DEX_BYTECODEMETHOD.instr) pc with
+        | None => true
+        | Some (ins,(op,l)) => 
+          for_all _
+          (fun (oj:option DEX_PC) => test oj)
+          (get_steps pc ins op)
+      end.
+
+    Lemma for_all_succs_bm_true : forall bm,
+      DEX_METHOD.body m = Some bm ->
+      for_all_succs_bm bm = true ->
+      forall ins oj,
+        instructionAt m pc = Some ins ->
+        DEX_step pc ins oj -> test oj = true.
+    Proof.
+      unfold for_all_succs_bm; intros.
+      assert (T2:=all_step_in_get_steps _ _ _ H2).
+      unfold instructionAt, DEX_BYTECODEMETHOD.instructionAt in H1.
+      rewrite H in H1.
+      caseeq (MapN.get (DEX_Instruction * (option DEX_PC*list DEX_ClassName)) (DEX_BYTECODEMETHOD.instr bm) pc).
+      intros (ins0,next0) T3.
+      rewrite T3 in H1; rewrite T3 in H0.
+      destruct next0.
+      apply for_all_true with
+        (test:=(fun oj : option DEX_PC => test oj))
+        (2:=T2).
+      unfold next, DEX_BYTECODEMETHOD.nextAddress.
+      inversion_mine H1.
+      rewrite H; rewrite T3; simpl; auto.
+      intros.
+      rewrite H3 in H1; discriminate.
+    Qed.
+
+  Definition for_all_succs_m : bool :=
+    match DEX_METHOD.body m with
+      | None => false
+      | Some bm => for_all_succs_bm bm
+    end.
+
+  Lemma for_all_succs_m_true : for_all_succs_m = true ->
+      forall ins oj,
+        instructionAt m pc = Some ins ->
+        DEX_step pc ins oj -> test oj = true.
+  Proof.
+    unfold for_all_succs_m.
+    generalize for_all_succs_bm_true.
+    destruct (DEX_METHOD.body m) as [bm|]; intro.
+    apply H; auto.
+    intros; discriminate.
+  Qed.
+   
+ End for_all_succs.
+
+
+  Section for_all_instrs.
+    Variable test : DEX_PC -> DEX_Instruction -> bool.
+
+    Definition for_all_instrs_bm (bm:DEX_BytecodeMethod) : bool :=
+      MapN.for_all _
+      (fun i (ins_next:DEX_Instruction*(option DEX_PC*list DEX_ClassName)) =>
+        let (ins,next) := ins_next in test i ins)
+      bm.(DEX_BYTECODEMETHOD.instr).
+
+    Lemma for_all_instrs_bm_true : forall bm,
+      DEX_METHOD.body m = Some bm ->
+      for_all_instrs_bm bm = true ->
+      forall i ins,
+        instructionAt m i = Some ins -> test i ins = true.
+    Proof.
+      intros.
+      assert (T1:=MapN.for_all_true _ _ _ H0).
+      unfold instructionAt, DEX_BYTECODEMETHOD.instructionAt in H1.
+      rewrite H in H1.
+      caseeq (MapN.get (DEX_Instruction * (option DEX_PC*list DEX_ClassName)) (DEX_BYTECODEMETHOD.instr bm) i).
+      intros (ins0,next0) T3.
+      rewrite T3 in H1.
+      generalize (T1 _ _ T3); clear T1; intros T1.
+      inversion_mine H1; auto.
+      intros T3; rewrite T3 in H1; discriminate.
+    Qed.
+
+    Definition for_all_instrs_m : bool :=
+      match DEX_METHOD.body m with
+        | None => false
+        | Some bm => for_all_instrs_bm bm
+      end.
+
+    Lemma for_all_instrs_m_true : for_all_instrs_m = true ->
+      forall i ins,
+        instructionAt m i = Some ins -> test i ins = true.
+    Proof.
+      unfold for_all_instrs_m.
+      generalize for_all_instrs_bm_true.
+      destruct (DEX_METHOD.body m) as [bm|]; intro.
+      apply H; auto.
+      intros; discriminate.
+    Qed.
+
+  End for_all_instrs.
+
+End DEX_S_section.
+
+Module DEX_MapClassTools := MapProjTools DEX_PROG.DEX_MapClass.
+
+Section p.
+  Variable p : DEX_Program.
+
+  Definition ValidMethod (m:DEX_Method) : Prop :=
+    exists c, DEX_PROG.defined_Class p c /\ DEX_CLASS.defined_Method c m.
+
+  Variable test : DEX_Method -> bool.
+
+  Definition for_all_methods : bool :=
+    DEX_MapClassTools.for_all
+    (fun cl =>  DEX_MapShortMethSign.for_all _ (fun _ => test) cl.(DEX_CLASS.methods))
+    p.(DEX_PROG.classes_map).
+
+  Lemma for_all_methods_true : for_all_methods = true ->
+    forall m, ValidMethod m -> test m = true.
+  Proof.
+    intros.
+    destruct H0 as [c [H0 H1]].
+    generalize (DEX_MapClassTools.for_all_true _ _ H _ H0); intros.
+    unfold DEX_CLASS.defined_Method, DEX_CLASS.method in H1.
+    caseeq (DEX_MapShortMethSign.get DEX_Method (DEX_CLASS.methods c) (DEX_METHOD.signature m)); intros.
+    rewrite H3 in H1.
+    destruct (DEX_METHODSIGNATURE.eq_t (DEX_METHOD.signature m) (DEX_METHOD.signature d)); inversion_mine H1.
+    apply (DEX_MapShortMethSign.for_all_true _ _ _ H2 _ _ H3).
+    rewrite H3 in H1; discriminate.
+  Qed.
+
+End p.
