DEX_I/DEX_typing_rules.v
@@ -1,0 +1,536 @@
+(** typing_rules.v: Typing rules, plus an executable type checker *)
+(* Hendra : - Modified to suit DEX program. 
+            - DEX has different instructions list from JVM.
+            - Also trim the system to contain only Arithmetic *)
+Require Export DEX_BigStepAnnot.
+Require Export Bool.
+Require Export DEX_step.
+Import DEX_BigStep.DEX_BigStep DEX_Dom.DEX_Prog.
+
+Import Level.L.
+Import DEX_Dom.
+
+Open Scope type_scope.
+
+  Section DEX_typing_rules.   (** Typing rules **)
+    Variable m : DEX_Method.
+    Variable sgn : DEX_sign.
+    Variable region : DEX_PC -> DEX_PC -> Prop.
+    Variable se : DEX_PC -> L.t.
+    Variable selift : DEX_PC -> L.t -> bool. 
+    Variable ret : DEX_Reg.
+
+    Infix "<=" := L.leql (at level 70).
+    Infix "<='" := L.leql' (at level 70).
+    Infix "U'" := L.join' (at level 60, right associativity).
+    Infix "U" := L.join (at level 60, right associativity).
+
+    Inductive texec : DEX_PC -> DEX_Instruction -> TypeRegisters -> option TypeRegisters -> Prop :=
+    | DEX_nop : forall i rt,
+      texec i DEX_Nop rt (Some rt)
+
+    | DEX_move : forall i (rt:TypeRegisters) k_rs (k:DEX_ValKind) (r:DEX_Reg) (rs:DEX_Reg),
+      In r (VarMap.dom _ rt) ->
+      In rs (VarMap.dom _ rt) ->
+      VarMap.get _ rt rs = Some k_rs ->
+      texec i (DEX_Move k r rs) rt
+        (Some (VarMap.update _ rt r ((se i) U k_rs)))
+
+    | DEX_return_ : forall i (rt:TypeRegisters),
+      sgn.(DEX_resType) = None ->
+      texec i (DEX_Return) rt None
+
+    | DEX_vReturn : forall i (rt:TypeRegisters) k_r kv (k:DEX_ValKind) (r:DEX_Reg),
+      In r (VarMap.dom _ rt) ->
+      VarMap.get _ rt r = Some k_r ->
+      sgn.(DEX_resType) = Some kv ->
+      ((se i) U k_r) <= kv -> 
+      texec i (DEX_VReturn k r) rt None
+
+    | DEX_const : forall i (rt:TypeRegisters) (k:DEX_ValKind) (r:DEX_Reg) (v:Z),
+      In r (VarMap.dom _ rt) ->
+      texec i (DEX_Const k r v) rt (Some (VarMap.update _ rt r (L.Simple (se i))))
+    
+    | DEX_goto : forall i (rt:TypeRegisters) (o:DEX_OFFSET.t),
+      texec i (DEX_Goto o) rt (Some rt)
+(* Hendra 11082016 focus on DEX I
+    | DEX_packedSwitch : forall i k (rt:TypeRegisters) (r:DEX_Reg) (firstKey:Z) (size:nat) (l:list DEX_OFFSET.t),
+      VarMap.get _ rt r = Some k ->
+      (forall j, region i None j -> k <= se j) -> 
+      texec i (DEX_PackedSwitch r firstKey size l) None rt (Some (lift_rt k rt))
+
+    | DEX_sparseSwitch : forall i k (rt:TypeRegisters) (r:DEX_Reg) (size:nat) (l:list (Z * DEX_OFFSET.t)),
+      VarMap.get _ rt r = Some k ->
+      (forall j, region i None j -> k <= se j) -> 
+      texec i (DEX_SparseSwitch r size l) None rt (Some (lift_rt k rt))
+*)
+
+    | DEX_ifcmp : forall i ka kb (rt:TypeRegisters) (cmp:DEX_CompInt) (ra:DEX_Reg) (rb:DEX_Reg) (o:DEX_OFFSET.t),
+      In ra (VarMap.dom _ rt) ->
+      In rb (VarMap.dom _ rt) ->
+      VarMap.get _ rt ra = Some ka ->
+      VarMap.get _ rt rb = Some kb ->
+      (forall j, region i j -> (ka U kb) <= se j) -> 
+      texec i (DEX_Ifcmp cmp ra rb o) rt (Some rt)
+     
+    | DEX_ifz : forall i k (rt:TypeRegisters) (cmp:DEX_CompInt) (r:DEX_Reg) (o:DEX_OFFSET.t),
+      In r (VarMap.dom _ rt) ->
+      VarMap.get _ rt r = Some k ->
+      (forall j, region i j -> k <= se j) -> 
+      texec i (DEX_Ifz cmp r o) rt (Some rt)
+
+    | DEX_ineg : forall i ks (rt:TypeRegisters) (r:DEX_Reg) (rs:DEX_Reg),
+      In r (VarMap.dom _ rt) ->
+      In rs (VarMap.dom _ rt) ->
+      VarMap.get _ rt rs = Some ks ->
+      texec i (DEX_Ineg r rs) rt (Some (VarMap.update _ rt r (L.Simple ((se i) U ks))))
+
+    | DEX_inot : forall i ks (rt:TypeRegisters) (r:DEX_Reg) (rs:DEX_Reg),
+      In r (VarMap.dom _ rt) ->
+      In rs (VarMap.dom _ rt) ->
+      VarMap.get _ rt rs = Some ks ->
+      texec i (DEX_Inot r rs) rt (Some (VarMap.update _ rt r (L.Simple ((se i) U ks))))
+
+    | DEX_i2b : forall i ks (rt:TypeRegisters) (r:DEX_Reg) (rs:DEX_Reg),
+      In r (VarMap.dom _ rt) ->
+      In rs (VarMap.dom _ rt) ->
+      VarMap.get _ rt rs = Some ks ->
+      texec i (DEX_I2b r rs) rt (Some (VarMap.update _ rt r (L.Simple ((se i) U ks))))
+
+    | DEX_i2s : forall i ks (rt:TypeRegisters) (r:DEX_Reg) (rs:DEX_Reg),
+      In r (VarMap.dom _ rt) ->
+      In rs (VarMap.dom _ rt) ->
+      VarMap.get _ rt rs = Some ks ->
+      texec i (DEX_I2s r rs) rt (Some (VarMap.update _ rt r (L.Simple ((se i) U ks))))
+
+    | DEX_ibinop : forall i ka kb (rt:TypeRegisters) (op:DEX_BinopInt) (r:DEX_Reg) (ra:DEX_Reg) (rb:DEX_Reg),
+      In r (VarMap.dom _ rt) ->
+      In ra (VarMap.dom _ rt) ->
+      In rb (VarMap.dom _ rt) ->
+      VarMap.get _ rt ra = Some ka ->
+      VarMap.get _ rt rb = Some kb ->
+      texec i (DEX_Ibinop op r ra rb) rt 
+       (Some (VarMap.update _ rt r (L.Simple ((ka U kb) U (se i)))))
+    
+    | DEX_ibinopConst : forall i ks (rt:TypeRegisters) (op:DEX_BinopInt) (r:DEX_Reg) (rs:DEX_Reg) (v:Z),
+      In r (VarMap.dom _ rt) ->
+      In rs (VarMap.dom _ rt) ->
+      VarMap.get _ rt rs = Some ks ->
+      texec i (DEX_IbinopConst op r rs v) rt 
+       (Some (VarMap.update _ rt r (L.Simple (ks U (se i)))))   
+    .
+
+    Section DEX_RT.
+      Variable RT : DEX_PC -> TypeRegisters.
+
+    Definition tsub_next (i:DEX_PC) (rt:TypeRegisters) : bool :=
+      match next m i with
+        | Some j => tsub_rt rt (RT j)
+        | None => false
+      end.
+
+    Fixpoint in_test (e:DEX_Reg) (l:list DEX_Reg) : bool :=
+      match l with
+        | nil => false
+        | cn::q => (Neq e cn) || (in_test e q)
+      end.
+
+    Lemma In_in_test_true : forall e l,
+      In e l -> in_test e l = true.
+    Proof.
+      induction l; simpl; intros.
+      elim H.
+      destruct H; subst.
+      generalize (Neq_spec e e).
+      destruct (Neq e e) ; simpl; auto.
+      rewrite IHl; auto.
+      destruct (Neq e a) ; simpl; auto.
+    Qed.
+
+    Lemma in_test_true_In : forall e l,
+      in_test e l = true -> In e l.
+    Proof.
+      induction l; simpl; intros.
+      inversion H.
+      apply orb_prop in H.
+      elim H; intros.
+      generalize (Neq_spec e a). intros. rewrite H0 in H1. left; symmetry; auto. 
+      right.
+      apply IHl; auto.
+    Qed.
+
+    Ltac clean_in_test :=
+      try match goal with
+        [ id1 : In ?e ?l, id2 : context[in_test ?e ?l = true] |- _ ] =>
+          rewrite (In_in_test_true e l id1) in id2
+      | [ id2 : context[in_test ?e ?l] |- _ ] =>
+          rewrite (In_in_test_true e l) in id2; [idtac|assumption]
+      end.
+
+    Definition tcompat_op (ot:option DEX_type) (ok:option L.t') : bool :=
+      match ot,ok with
+        | None,None => true
+        | Some _,Some _ => true
+        | _,_ => false
+      end.
+
+    Lemma tcompat_op_true : forall (ot:option DEX_type) (ok:option L.t'),
+      tcompat_op ot ok = true -> compat_op ot ok.
+    Proof.
+      destruct ot; destruct ok; simpl; intros; discriminate || constructor.
+    Qed.
+
+    Fixpoint le_nat_test (n1 n2:nat) {struct n1} : bool :=
+       match n1 with
+         | O => true
+         | Datatypes.S p1 =>
+             match n2 with
+               | O => false
+               | Datatypes.S p2 => le_nat_test p1 p2
+             end
+       end.
+
+    Lemma le_nat_test_correct : forall n1 n2,
+      if le_nat_test n1 n2 then (n1<=n2)%nat else (~(n1<=n2))%nat.
+    Proof.
+      induction n1; simpl.
+      intros; omega.
+      destruct n2; simpl.
+      omega.
+      generalize (IHn1 n2); destruct (le_nat_test n1 n2); omega.
+    Qed.
+
+    Lemma le_nat_test_true : forall n1 n2,
+      le_nat_test n1 n2 = true -> (n1<=n2)%nat.
+    Proof.
+      intros.
+      generalize (le_nat_test_correct n1 n2).
+      rewrite H; auto.
+    Qed.
+
+   Lemma Reg_eq_dec : forall x y : DEX_Reg, {x=y} + {x<>y}.
+   Proof.
+    repeat decide equality.
+   Qed.
+
+   Definition DEX_tcheck (i:DEX_PC) (ins:DEX_Instruction) : bool :=
+      match ins, RT i with
+        | DEX_Nop, rt1 =>
+          tsub_next i rt1
+
+        | DEX_Move _ r rs, rt1 =>
+          in_test rs (VarMap.dom _ rt1) && in_test r (VarMap.dom _ rt1) && 
+          match VarMap.get _ rt1 rs with
+            | Some k_rs =>
+                tsub_next i (VarMap.update _ rt1 r (L.join (se i) (k_rs)))
+            | None => false
+          end
+
+        | DEX_Return, rt1 =>
+          match sgn.(DEX_resType) with
+            | None => true
+            | _ => false
+          end
+
+        | DEX_VReturn _ r, rt1 =>          
+          in_test r (VarMap.dom _ rt1) && 
+          match sgn.(DEX_resType) with
+            | None => false
+            | Some kv => 
+              match VarMap.get _ rt1 r with
+                | None => false
+                | Some k => leql_t (se i U k) kv 
+              end
+          end
+
+        | DEX_Const _ r _, rt1 =>
+          in_test r (VarMap.dom _ rt1) && 
+          tsub_next i (VarMap.update _ rt1 r (L.Simple (se i)))
+
+        | DEX_Goto o, rt1 => tsub_rt rt1 (RT (DEX_OFFSET.jump i o))
+
+      (* Hendra 11082016 focus on DEX I - 
+        | DEX_PackedSwitch r _ _ l, rt1 =>
+          match VarMap.get _ rt1 r with
+            | None => false
+            | Some k => (selift i None k) && (tsub_next i (lift_rt k rt1)) &&
+               (for_all _
+                 (fun o => tsub_rt (lift_rt k rt1) (RT ((*DEX_OFFSET.*)jumpAddress i o))) l)  
+          end
+   
+        | DEX_SparseSwitch r _ l, rt1 =>
+          match VarMap.get _ rt1 r with
+            | None => false
+            | Some k => (selift i None k) && (tsub_next i (lift_rt k rt1)) &&
+               (for_all _
+                 (fun o => tsub_rt (lift_rt k rt1) (RT ((*DEX_OFFSET.*)jumpAddress i o)))
+                 (@map _ _ (@snd _ _) l))
+          end
+      *)    
+        | DEX_Ifcmp _ ra rb o, rt1 =>
+          in_test ra (VarMap.dom _ rt1) && in_test rb (VarMap.dom _ rt1) && 
+          match VarMap.get _ rt1 ra, VarMap.get _ rt1 rb with
+            | Some ka, Some kb =>
+                (selift i (ka U kb)) && 
+                (tsub_next i rt1) &&
+                (tsub_rt rt1 (RT (DEX_OFFSET.jump i o)))
+            | _, _ => false
+          end
+
+        | DEX_Ifz _ r o, rt1 =>
+          in_test r (VarMap.dom _ rt1) && 
+          match VarMap.get _ rt1 r with
+            | Some k => 
+                (selift i k) && 
+                (tsub_next i rt1) &&
+                (tsub_rt rt1 (RT (DEX_OFFSET.jump i o)))
+            | None => false
+          end        
+
+        | DEX_Ineg r rs, rt1 =>
+          in_test rs (VarMap.dom _ rt1) && in_test r (VarMap.dom _ rt1) && 
+          match VarMap.get _ rt1 rs with
+            | Some ks => (tsub_next i (VarMap.update _ rt1 r (L.Simple ((se i) U ks))) )
+            | None => false
+          end   
+
+        | DEX_Inot r rs, rt1 =>
+          in_test rs (VarMap.dom _ rt1) && in_test r (VarMap.dom _ rt1) && 
+          match VarMap.get _ rt1 rs with
+            | Some ks => (tsub_next i (VarMap.update _ rt1 r (L.Simple ((se i) U ks))) )
+            | None => false
+          end   
+
+        | DEX_I2b r rs, rt1 =>
+          in_test rs (VarMap.dom _ rt1) && in_test r (VarMap.dom _ rt1) && 
+          match VarMap.get _ rt1 rs with
+            | Some ks => (tsub_next i (VarMap.update _ rt1 r (L.Simple ((se i) U ks))) )
+            | None => false
+          end
+
+        | DEX_I2s r rs, rt1 =>
+          in_test rs (VarMap.dom _ rt1) && in_test r (VarMap.dom _ rt1) && 
+          match VarMap.get _ rt1 rs with
+            | Some ks => (tsub_next i (VarMap.update _ rt1 r (L.Simple ((se i) U ks))) )
+            | None => false
+          end   
+
+        | DEX_Ibinop _ r ra rb, rt1 =>
+          in_test r (VarMap.dom _ rt1) && in_test ra (VarMap.dom _ rt1) && in_test rb (VarMap.dom _ rt1) && 
+          match VarMap.get _ rt1 ra, VarMap.get _ rt1 rb with
+            | Some ka, Some kb => 
+               (tsub_next i (VarMap.update _ rt1 r (L.Simple ((ka U kb) U (se i)))) )
+            | _, _ => false
+          end   
+
+        | DEX_IbinopConst _ r rs _, rt1 =>
+          in_test rs (VarMap.dom _ rt1) && in_test r (VarMap.dom _ rt1) && 
+          match VarMap.get _ rt1 rs with
+            | Some ks => (tsub_next i (VarMap.update _ rt1 r (L.Simple (ks U (se i)))) )
+            | None => false
+          end   
+      end.
+
+   Ltac flatten_bool :=
+     repeat match goal with
+       [ id : _ && _ = true |- _ ] =>  destruct (andb_prop _ _ id); clear id
+     end.
+
+   Variable selift_prop : forall i  k,
+     selift i k = true ->
+     forall j, region i j -> k <= (se j).
+
+   Ltac replace_selift :=
+     repeat match goal with
+       [ id : selift _ _ = true |- _ ] =>  
+         generalize (selift_prop _ _ id);
+           clear id; intros id
+     end.
+
+   Lemma leql_prop : forall x y,
+     L.leql_t x y = true -> x <= y.
+   Proof.
+     intros.
+     generalize (L.leql_t_spec x y); rewrite H; auto.
+   Qed.
+
+   Ltac replace_leql :=
+     repeat match goal with
+       [ id : L.leql_t _ _ = true |- _ ] =>  
+         generalize (leql_prop _ _ id);
+           clear id; intros id
+     | [ id : leql'_test ?x ?y = true |- _ ] =>  
+       generalize (leql'_test_prop x y); rewrite id; clear id; intros id
+     end.
+
+   Ltac replace_for_all :=
+     match goal with
+       [ id1 : for_all _ _ ?l = true,
+         id2 : In ?e ?l |- _] =>
+       generalize (for_all_true _ _ _ id1 _ id2);
+         clear id1; intros id1
+     end.
+
+   Ltac flatten :=
+     flatten_bool; try replace_for_all; flatten_bool; replace_selift; clean_in_test; replace_leql.
+
+   Lemma length_le_app_form : forall (A:Set) n (l:list A),
+     (n<= length l)%nat -> exists l1, exists l2,
+       l = l1++l2 /\ n = length l1.
+   Proof.
+     induction n; intros.
+     exists (@nil A); exists l; split; auto.
+     inversion H.
+     exists l; exists (@nil A); split; auto.
+     apply app_nil_end.
+     elim IHn with l.
+     intros l1 [l2 [H3 H2]].
+     destruct l2.
+     rewrite <- app_nil_end in H3; subst.
+     apply False_ind; omega.
+     exists (l1++(a::nil)); exists l2; split.
+     rewrite <- app_cons; auto.
+     rewrite length_app_cons_nil; congruence.
+     omega.
+   Qed.
+
+   Ltac split_match :=
+     repeat 
+       match goal with
+         | [ _ : context[match ?x with nil => _ | _ :: _ => _ end] |- _] => destruct x
+         | [ _ : context[match ?x with L.Simple _ => _ | L.Array _ _ => _ end] |- _] => destruct x
+         | [_ :  context [match ?x with
+                            | DEX_Make.DEX_AddInt => _
+                            | DEX_Make.DEX_AndInt => _
+                            | DEX_Make.DEX_DivInt => _
+                            | DEX_Make.DEX_MulInt => _
+                            | DEX_Make.DEX_OrInt => _
+                            | DEX_Make.DEX_RemInt => _
+                            | DEX_Make.DEX_ShlInt => _
+                            | DEX_Make.DEX_ShrInt => _
+                            | DEX_Make.DEX_SubInt => _
+                            | DEX_Make.DEX_UshrInt => _
+                            | DEX_Make.DEX_XorInt => _
+                          end] |- _] => destruct x
+       end.
+
+   Lemma tcheck_correct1 : forall i ins,
+     DEX_tcheck i ins = true ->
+      DEX_step m i ins None -> texec i ins (RT i) None.
+   Proof.
+     intros.
+     inversion_clear H0 in H;
+       unfold DEX_tcheck in *.
+     (* Return *)
+     try discriminate; flatten; constructor; auto.
+     destruct (DEX_resType sgn); congruence.
+
+     (* VReturn *)
+     apply andb_prop in H; inversion H as [H3 H4].
+     destruct (DEX_resType sgn) eqn:H1.
+     destruct (VarMap.get t (RT i) rt) eqn:H2. 
+     apply DEX_vReturn with (k_r:=t1) (kv:=t0); auto.
+      apply VarMap.get_some_in_dom.
+      unfold not; intros. rewrite H0 in H2. inversion H2.
+
+    generalize (leql_t_spec (se i U t1) t0); intros.
+    rewrite H4 in H0; auto.
+     inversion H4.
+     inversion H4.
+   Qed.
+
+   Ltac replace_tsub_next :=
+     try match goal with
+       [ id1 : tsub_next _ ?rt = true, id2 : next _ _ = _ |- _ ] =>
+         unfold tsub_next in id1; rewrite id2 in id1
+     end.
+
+   Ltac search_tsub :=
+     match goal with
+       [ id1 : tsub_rt ?rt (RT _) = true |- _ ] =>
+         exists rt; split; [clear id1 | exact id1]
+         end.
+
+   Ltac flatten2 := flatten; replace_tsub_next; search_tsub.
+
+   Hint Constructors texec : texec.
+
+   Lemma tcheck_correct2 : forall i ins,
+     DEX_tcheck i ins = true ->
+     forall j, DEX_step m i ins (Some j) ->
+       exists rt,
+       texec i ins (RT i) (Some rt)
+       /\ tsub_rt rt (RT j) = true.
+   Proof.
+     intros.
+     inversion_clear H0 in H;
+       unfold DEX_tcheck in *;
+        try (split_match; intuition; subst; try discriminate; 
+         flatten2; eauto with texec; fail); 
+    try (flatten; destruct (VarMap.get _ (RT i) rs) eqn:Hrs; try (inversion H2; fail);
+    flatten2; constructor; try (apply in_test_true_In); auto; fail).
+    
+    (* const *)
+    flatten2; constructor; try (apply in_test_true_In); auto.
+
+     (* Ifcmp *)
+     flatten.
+     destruct (VarMap.get t (RT i) ra) eqn:Hra; try (inversion H2; fail). 
+     destruct (VarMap.get t (RT i) rb) eqn:Hrb; try (inversion H2; fail).
+     flatten_bool; replace_selift. inversion H1.
+       (* next successor *)
+       replace_tsub_next; search_tsub.
+       apply DEX_ifcmp with (ka:=t0) (kb:=t1); try (apply in_test_true_In; auto; fail); auto. 
+       (* target successor *) 
+       rewrite H0. exists (RT i). split. 
+       apply DEX_ifcmp with (ka:=t0) (kb:=t1); auto; try (apply in_test_true_In; auto; fail).  
+       auto.
+     (* Ifz *)
+     flatten.
+     destruct (VarMap.get t (RT i) r) eqn:Hr; try (inversion H2; fail).
+     flatten_bool; replace_selift. inversion H1.
+       (* next successor *)
+       replace_tsub_next; search_tsub.
+       apply DEX_ifz with (k:=t0); auto; try (apply in_test_true_In; auto; fail). 
+       (* target successor *) 
+       rewrite H. exists (RT i). split. 
+       apply DEX_ifz with (k:=t0); auto; try (apply in_test_true_In; auto; fail). exact H3.
+
+     (* Ibinop *)
+     flatten.
+     destruct (VarMap.get t (RT i) ra) eqn:Hra. try (inversion H2; fail).
+     destruct (VarMap.get t (RT i) rb) eqn:Hrb; try (inversion H2; fail).
+     flatten2; apply DEX_ibinop; auto; try (apply in_test_true_In; auto; fail). inversion H2.
+     (* IbinopConst *)
+     flatten.
+     destruct (VarMap.get t (RT i) r) eqn:Hr; try (inversion H2; fail);
+     flatten2; apply DEX_ibinopConst; try (apply in_test_true_In; auto; fail); apply Hr.
+  (* Hendra 11082016 focus on DEX I - 
+     (* PackedSwitch *)
+     destruct (VarMap.get t' (RT i) rt) eqn:Hr; try (inversion H; fail).
+     flatten_bool; replace_selift. inversion H1. 
+       (* default successor *)
+       exists (lift_rt t0 (RT i)); split. apply DEX_packedSwitch.
+       apply Hr. apply H. inversion H0. unfold tsub_next in H3.
+        inversion H4.
+       rewrite_nextAddress.
+       rewrite H5 in H3. rewrite <- H6. apply H3.
+       (* other successors *)
+       exists (lift_rt t0 (RT i)); split. apply DEX_packedSwitch.
+       apply Hr. apply H. replace_for_all. apply H2.
+     (* SparseSwitch *)
+     destruct (VarMap.get t' (RT i) rt) eqn:Hr; try (inversion H; fail).
+     flatten_bool; replace_selift. inversion H1. 
+       (* default successor *)
+       exists (lift_rt t0 (RT i)); split. apply DEX_sparseSwitch.
+       apply Hr. apply H. inversion H0. unfold tsub_next in H3.
+       inversion H4.
+       rewrite_nextAddress. 
+       rewrite H5 in H3. rewrite <- H6. apply H3.
+       (* other successors *)
+       exists (lift_rt t0 (RT i)); split. apply DEX_sparseSwitch.
+       apply Hr. apply H. replace_for_all. apply H2.
+*)
+   Qed.
+ End DEX_RT.
+End DEX_typing_rules.
