DEX_I/cdr.v
@@ -1,0 +1,30 @@
+(** * cdr.v: Control Dependence Region (interface) *)
+(* Hendra : Removed exception related SOAP *)
+Set Implicit Arguments.
+Section GRAPH.
+
+  Variable PC Tag: Set.
+  Variable step : PC -> option PC -> Prop.
+  Definition result p := step p None.
+
+  Record CDR : Type := make_CDR {
+     region : PC -> PC -> Prop;
+     junc : PC -> PC -> Prop;
+     junc_func: forall i j1 j2,
+       junc i j1 -> junc i j2 -> j1=j2;
+     soap1: forall i j k,
+       step i (Some j) ->
+       step i (Some k) ->
+       j <> k ->
+       region i k \/ junc i k;
+     soap2:forall i j k,
+       region i j-> 
+       step j (Some k) ->
+       region i k \/ junc i k;
+     soap3 : forall i j k, 
+       region i j -> 
+       result j -> 
+       ~ junc i k
+  }.
+
+End GRAPH.
