DEX_I/check_cdr.v
@@ -1,0 +1,359 @@
+(** * check_cdr.v: executable CDR checker *)
+(* Hendra : Removed exception related SOAP *)
+Require Export Lib.
+Require Export cdr.
+Require Export ZArith.
+
+Module Make (M:MAP).
+
+  Section region.
+
+    Definition PC : Set := M.key.
+
+    Variable step : PC -> option PC -> Prop.
+    Variable for_all_steps : (PC -> option PC->bool)  -> bool.
+    Variable test_all_steps : (PC -> option PC->bool)  -> list (PC*bool).
+    Variable for_all_steps_true : 
+      forall test, for_all_steps test  = true ->
+        forall i oj,
+          step i oj -> test i oj = true.
+    Variable for_all_succs : PC -> (option PC -> bool) -> bool.
+    Variable for_all_succs_true : forall i test,
+      for_all_succs i test = true ->
+      forall oj, step i oj -> test oj = true.
+    
+    Definition result p := step p None.
+
+    Variable reg : M.t (M.t bool).
+    Variable jun : M.t PC.
+
+    Definition region (i:PC) (j:PC) : Prop :=
+      exists m,
+        M.get reg (i) = Some m
+        /\ M.get m j = Some true.
+
+    Definition junc (i:PC) (j:PC) : Prop :=
+      M.get jun (i) = Some j.
+    
+    Definition check_junc_func : bool :=
+      M.for_all
+        (fun i j1 => 
+          match M.get jun i with
+            | None => true
+            | Some j2 =>  M.eq_key j1 j2
+          end) jun.
+
+    Lemma check_junc_func_correct : check_junc_func = true ->
+      forall i j1 j2,
+        junc i j1 -> junc i j2 -> j1=j2.
+    Proof.
+      unfold check_junc_func, junc; intros.
+      generalize (M.for_all_true _ _ _ H _ _ H0); simpl.
+      rewrite H1; intros.
+      generalize (M.eq_key_spec j1 j2); rewrite H2; auto.    
+    Qed.
+    
+    Definition in_region (i:PC) (j:PC) : bool :=
+      match M.get reg (i) with
+        | None => false
+        | Some m => match M.get m j with
+                      | Some true => true
+                      | _ => false
+                    end
+      end.
+
+    Lemma in_region_true : forall i j,
+      in_region i j = true -> region i j.
+    Proof.
+      unfold in_region, region; intros i j.
+      destruct (M.get reg (i)); try (intros; discriminate).
+      case_eq (M.get t j); try (intros; discriminate).
+      destruct b; intros; try discriminate.
+      eauto.
+    Qed.
+
+    Definition test_junc (i:PC) (j:PC) : bool :=
+      match M.get jun (i) with
+        | None => false
+        | Some j0 => M.eq_key j0 j
+      end.
+
+    Lemma test_junc_true : forall i j,
+      test_junc i j = true -> junc i j.
+    Proof.
+      unfold test_junc, junc; intros i j.
+      destruct (M.get jun (i)); intros; try discriminate.
+      generalize (M.eq_key_spec p j); rewrite H; congruence.
+    Qed.
+    
+     Definition check_soap1 : bool :=
+      for_all_steps
+        (fun i oj =>
+          for_all_steps (fun i ok =>
+            match oj, ok with
+              | Some j, Some k => orb (M.eq_key j k) (orb (in_region i k) (test_junc i k))
+              | _, _ => false
+            end)). 
+
+    Definition check_soap1' : list (PC*bool) :=
+      test_all_steps
+        (fun i oj =>
+          for_all_steps (fun i ok =>
+          match oj, ok with
+            | None, NOne => true 
+            | Some j, Some k => orb (M.eq_key j k) (orb (in_region i j) (test_junc i j))
+            | _, _ => false
+          end)).
+        
+    Lemma check_soap1_correct : check_soap1 = true ->
+      forall i j k,
+        step i (Some j) -> step i (Some k) -> j <> k ->
+        region i k \/ junc i k.
+    Proof.
+      unfold check_soap1; intros.
+      assert (T:=for_all_steps_true _ H _ _ H0); simpl in T.
+      assert (T':=for_all_steps_true _ T _ _ H1); simpl in T'.
+      elim orb_prop with (1:=T'); intros.
+        generalize (M.eq_key_spec j k). rewrite H3; congruence.
+      elim orb_prop with (1:=H3); intros.
+      left; apply in_region_true; auto.
+      right; apply test_junc_true; auto.
+    Qed.
+
+    Definition for_all_region (test:PC->PC->bool) : bool :=
+      M.for_all
+        (fun i m => 
+           M.for_all 
+             (fun j b => (negb b) || test i j)
+             m)
+        reg.
+
+    Lemma for_all_region_true : forall test,
+      for_all_region test = true ->
+      forall i j, region i j -> test i j = true.
+    Proof.
+      unfold for_all_region, region; intros.
+      destruct H0 as [m [H0 H1]].
+      assert (T:=M.for_all_true _ _ _ H _ _ H0).
+      elim orb_prop with (1:=M.for_all_true _ _ _ T _ _ H1); auto.
+      intros; discriminate.
+    Qed.
+
+    Definition for_all_region1 (i0:PC) (test:PC->bool) : bool :=
+      M.for_all
+        (fun i m => 
+           negb (M.eq_key i0 i) ||
+           M.for_all 
+             (fun j b => (negb b) || test j)
+             m)
+        reg.
+
+    Lemma for_all_region1_true : forall i test,
+      for_all_region1 i test = true ->
+      forall j, region i j -> test j = true.
+    Proof.
+      unfold for_all_region1, region; intros.
+      destruct H0 as [m [H0 H1]].
+      assert (T:=M.for_all_true _ _ _ H _ _ H0).
+      simpl in T.
+      elim orb_prop with (1:=T); intros.
+      generalize (M.eq_key_spec i i); destruct (M.eq_key i i); simpl in *; intros.
+      discriminate.
+      elim H3; auto.
+      elim orb_prop with (1:=M.for_all_true _ _ _ H2 _ _ H1); auto.
+      intros; discriminate.
+    Qed.
+
+
+    Definition for_all_region2 (i:PC) (test:PC->bool) : bool :=
+      match M.get reg (i) with
+        | None => true
+        | Some m => M.for_all (fun j b => b && test j) m
+      end.
+
+    Lemma for_all_region2_true : forall test i,
+      for_all_region2 i test = true ->
+      forall j, region i j -> test j = true.
+    Proof.
+      unfold for_all_region2, region; intros.
+      destruct H0 as [m [H0 H1]].
+      rewrite H0 in H.
+      assert (T:=M.for_all_true _ _ _ H _ _ H1).
+      auto.
+    Qed.
+
+    Definition check_soap2 : bool := 
+      for_all_region
+        (fun i j =>
+          for_all_succs j
+            (fun ok => 
+              match ok with
+                | None => true
+                | Some k => orb (in_region i k) (test_junc i k)
+              end)).
+
+    Lemma check_soap2_correct : check_soap2 = true ->
+      forall i j k,
+        region i j-> 
+        step j (Some k) ->
+        region i k \/ junc i k.
+    Proof.
+      unfold check_soap2; intros.
+      generalize (for_all_region_true _ H _ _ H0); intros T.
+      elim orb_prop with (1:=for_all_succs_true _ _ T _ H1); intros.
+      left; apply in_region_true; auto.
+      right; apply test_junc_true; auto.
+    Qed.
+
+    Definition test_all_region (test:PC->PC->bool) : list (PC*PC) :=
+      M.fold 
+        (fun i m l =>
+            M.fold
+              (fun j (b:bool) l =>
+                if b then 
+                  (if test i j then l else (i,j)::l)
+                  else l)
+              m l)
+        reg nil.
+
+    Definition test_soap2 : list (PC*PC) := 
+      test_all_region
+        (fun i j =>
+          for_all_succs j
+            (fun ok => 
+              match ok with
+                | None => true
+                | Some k => orb (in_region i k) (test_junc i k)
+              end)).
+
+
+    Definition for_all_result (test:PC->bool) : bool :=
+      for_all_steps
+      (fun i oj => 
+        match oj with
+          | None => test i
+          | Some _ => true
+        end).
+
+    Lemma for_all_result_true : forall test, for_all_result test = true ->
+      forall i, result i -> test i = true.
+    Proof.
+      unfold for_all_result, result; intros.
+      apply (for_all_steps_true _ H _ _ H0).
+    Qed.
+
+    Definition for_all_junc (test:PC->PC->bool) : bool :=
+      M.for_all
+        (fun i j => 
+           test i j)
+        jun.
+
+    Lemma for_all_junc_true : forall test,
+      for_all_junc test = true ->
+      forall i j, junc i j -> test i j = true.
+    Proof.
+      unfold for_all_junc, junc; intros.
+      apply (M.for_all_true _ _ _ H _ _ H0).
+    Qed.
+
+    Definition for_all_junc1 (i0:PC) (test:PC->bool) : bool :=
+      M.for_all 
+        (fun i j => (negb (M.eq_key i i0)) || (test j))
+        jun.
+
+    Lemma for_all_junc1_true : forall i test,
+      for_all_junc1 i test = true ->
+      forall j, junc i j -> test j = true.
+    Proof.
+      unfold for_all_junc1, junc; intros.
+      elim orb_prop with (1:=M.for_all_true _ _ _ H _ _ H0); intros; auto.
+      generalize (M.eq_key_spec i i); destruct (M.eq_key i i); intuition.
+    Qed.
+
+    Definition check_soap3 : bool :=
+      for_all_junc
+      (fun i k => 
+        (match M.get reg (i) with
+           | None => true
+           | Some m => M.for_all 
+             (fun j b => 
+               (negb b) ||
+                 (for_all_succs j
+                   (fun ok => 
+                     match ok with
+                       | None => false
+                       | Some k => true
+                     end))) m
+         end)).
+
+    Lemma check_soap3_correct : check_soap3 = true ->
+      forall i j k, 
+       region i j -> 
+       result j -> 
+       ~ junc i k.
+    Proof.
+      unfold check_soap3, region, result; red; intros.
+      assert (HH:=(for_all_junc_true _ H _ _ H2)); clear H H2.
+      destruct H0 as [m [H H2]].
+      simpl in HH.
+      rewrite H in HH.
+      elim orb_prop with (1:=M.for_all_true _ _ _ HH _ _ H2); simpl; intros.
+      discriminate.
+      generalize (for_all_succs_true _ _ H0 _ H1); intros; discriminate.
+    Qed.
+
+    Definition check_soaps : bool :=
+      check_junc_func && 
+      check_soap1 && 
+      check_soap2 && 
+      check_soap3 (*&& 
+      check_soap4 && 
+      check_soap5 && 
+      check_soap5'*).
+
+    Definition check_soaps' :=
+      (check_junc_func,
+        check_soap1,
+        check_soap2, 
+        check_soap3).
+
+    Lemma check_soap_true :
+      check_soaps = true ->
+      { cdr : CDR step |
+        forall i j, cdr.region cdr i j -> region i j }.
+    Proof.
+      unfold check_soaps; intros; 
+        repeat match goal with
+                 [ id : _ && _ = true |- _ ] =>  destruct (andb_prop _ _ id); clear id
+               end.
+      exists (make_CDR step region junc
+               (check_junc_func_correct H0)
+               (check_soap1_correct H3)
+               (check_soap2_correct H2)
+               (check_soap3_correct H1)).
+      simpl; auto.    
+    Qed.
+
+    Definition for_all_in_region : PC -> (PC->bool) -> bool :=
+      fun i test =>
+        match M.get reg (i) with
+          | None => true
+          | Some m =>
+            M.for_all (fun j b => (negb b) || test j)
+            m
+        end.
+    Lemma for_all_in_region_correct : forall i test,
+      for_all_in_region i test = true ->
+      forall j, region i j -> test j = true.
+    Proof.
+      unfold region, for_all_in_region; intros.
+      destruct H0 as [m [H0 H1]].
+      rewrite H0 in H.
+      elim orb_prop with (1:=M.for_all_true _ _ _ H _ _ H1); simpl; intros.
+      discriminate.
+      auto.
+    Qed.
+
+  End region.
+
+End Make.
